QCP_examples/humaneval/spec_logic_rewrite_c_files/C_146_goal.v
@@ -1,0 +1,848 @@
+Require Import Coq.ZArith.ZArith.
+Require Import Coq.Bool.Bool.
+Require Import Coq.Strings.String.
+Require Import Coq.Strings.Ascii.
+Require Import Coq.Lists.List.
+Require Import Coq.Classes.RelationClasses.
+Require Import Coq.Classes.Morphisms.
+Require Import Coq.micromega.Psatz.
+Require Import Coq.Sorting.Permutation.
+From AUXLib Require Import int_auto Axioms Feq Idents ListLib VMap.
+Require Import SetsClass.SetsClass. Import SetsNotation.
+From SimpleC.SL Require Import Mem SeparationLogic.
+Require Import Logic.LogicGenerator.demo932.Interface.
+Local Open Scope Z_scope.
+Local Open Scope sets.
+Local Open Scope string_scope.
+Local Open Scope list.
+Import naive_C_Rules.
+Require Import coins_146.
+Local Open Scope sac.
+From SimpleC.EE.QCP_demos_LLM Require Import int_array_strategy_goal.
+From SimpleC.EE.QCP_demos_LLM Require Import int_array_strategy_proof.
+From SimpleC.EE.QCP_demos_LLM Require Import uint_array_strategy_goal.
+From SimpleC.EE.QCP_demos_LLM Require Import uint_array_strategy_proof.
+From SimpleC.EE.QCP_demos_LLM Require Import undef_uint_array_strategy_goal.
+From SimpleC.EE.QCP_demos_LLM Require Import undef_uint_array_strategy_proof.
+From SimpleC.EE.QCP_demos_LLM Require Import array_shape_strategy_goal.
+From SimpleC.EE.QCP_demos_LLM Require Import array_shape_strategy_proof.
+
+(*----- Function specialFilter -----*)
+
+Definition specialFilter_safety_wit_1 := 
+forall (nums_size_pre: Z) (nums_pre: Z) (input_l: (@list Z)) (PreH1 : (nums_pre <> 0)) (PreH2 : (0 <= nums_size_pre)) (PreH3 : (nums_size_pre < INT_MAX)) (PreH4 : (nums_size_pre = (Zlength (input_l)))) (PreH5 : (problem_146_pre_z input_l )) (PreH6 : (special_filter_safe_146 input_l )) ,
+  ((( &( "num" ) )) # Int  |->_)
+  **  ((( &( "nums_size" ) )) # Int  |-> nums_size_pre)
+  **  ((( &( "nums" ) )) # Ptr  |-> nums_pre)
+  **  (IntArray.full nums_pre nums_size_pre input_l )
+|--
+  “ (0 <= INT_MAX) ” 
+  &&  “ ((INT_MIN) <= 0) ”
+.
+
+Definition specialFilter_safety_wit_2 := 
+forall (nums_size_pre: Z) (nums_pre: Z) (input_l: (@list Z)) (PreH1 : (nums_pre <> 0)) (PreH2 : (0 <= nums_size_pre)) (PreH3 : (nums_size_pre < INT_MAX)) (PreH4 : (nums_size_pre = (Zlength (input_l)))) (PreH5 : (problem_146_pre_z input_l )) (PreH6 : (special_filter_safe_146 input_l )) ,
+  ((( &( "i" ) )) # Int  |->_)
+  **  ((( &( "num" ) )) # Int  |-> 0)
+  **  ((( &( "nums_size" ) )) # Int  |-> nums_size_pre)
+  **  ((( &( "nums" ) )) # Ptr  |-> nums_pre)
+  **  (IntArray.full nums_pre nums_size_pre input_l )
+|--
+  “ (0 <= INT_MAX) ” 
+  &&  “ ((INT_MIN) <= 0) ”
+.
+
+Definition specialFilter_safety_wit_3 := 
+forall (nums_size_pre: Z) (nums_pre: Z) (input_l: (@list Z)) (i: Z) (num: Z) (current: Z) (PreH1 : (0 <= nums_size_pre)) (PreH2 : (nums_size_pre < INT_MAX)) (PreH3 : (nums_size_pre = (Zlength (input_l)))) (PreH4 : (problem_146_pre_z input_l )) (PreH5 : (special_filter_safe_146 input_l )) (PreH6 : (0 <= i)) (PreH7 : (i < nums_size_pre)) (PreH8 : (0 <= num)) (PreH9 : (num <= i)) (PreH10 : (current = (Znth (i) (input_l) (0)))) (PreH11 : (INT_MIN <= current)) (PreH12 : (current <= INT_MAX)) (PreH13 : (special_filter_prefix_146 input_l i num )) ,
+  ((( &( "nums" ) )) # Ptr  |-> nums_pre)
+  **  ((( &( "nums_size" ) )) # Int  |-> nums_size_pre)
+  **  ((( &( "i" ) )) # Int  |-> i)
+  **  ((( &( "num" ) )) # Int  |-> num)
+  **  ((( &( "current" ) )) # Int  |-> current)
+  **  (IntArray.full nums_pre nums_size_pre input_l )
+|--
+  “ (10 <= INT_MAX) ” 
+  &&  “ ((INT_MIN) <= 10) ”
+.
+
+Definition specialFilter_safety_wit_4 := 
+forall (nums_size_pre: Z) (nums_pre: Z) (input_l: (@list Z)) (i: Z) (num: Z) (current: Z) (PreH1 : (current > 10)) (PreH2 : (0 <= nums_size_pre)) (PreH3 : (nums_size_pre < INT_MAX)) (PreH4 : (nums_size_pre = (Zlength (input_l)))) (PreH5 : (problem_146_pre_z input_l )) (PreH6 : (special_filter_safe_146 input_l )) (PreH7 : (0 <= i)) (PreH8 : (i < nums_size_pre)) (PreH9 : (0 <= num)) (PreH10 : (num <= i)) (PreH11 : (current = (Znth (i) (input_l) (0)))) (PreH12 : (INT_MIN <= current)) (PreH13 : (current <= INT_MAX)) (PreH14 : (special_filter_prefix_146 input_l i num )) ,
+  ((( &( "last" ) )) # Int  |->_)
+  **  ((( &( "first" ) )) # Int  |-> current)
+  **  ((( &( "nums" ) )) # Ptr  |-> nums_pre)
+  **  ((( &( "nums_size" ) )) # Int  |-> nums_size_pre)
+  **  ((( &( "i" ) )) # Int  |-> i)
+  **  ((( &( "num" ) )) # Int  |-> num)
+  **  ((( &( "current" ) )) # Int  |-> current)
+  **  (IntArray.full nums_pre nums_size_pre input_l )
+|--
+  “ ((current <> (INT_MIN)) \/ (10 <> (-1))) ” 
+  &&  “ (10 <> 0) ”
+.
+
+Definition specialFilter_safety_wit_5 := 
+forall (nums_size_pre: Z) (nums_pre: Z) (input_l: (@list Z)) (i: Z) (num: Z) (current: Z) (PreH1 : (current > 10)) (PreH2 : (0 <= nums_size_pre)) (PreH3 : (nums_size_pre < INT_MAX)) (PreH4 : (nums_size_pre = (Zlength (input_l)))) (PreH5 : (problem_146_pre_z input_l )) (PreH6 : (special_filter_safe_146 input_l )) (PreH7 : (0 <= i)) (PreH8 : (i < nums_size_pre)) (PreH9 : (0 <= num)) (PreH10 : (num <= i)) (PreH11 : (current = (Znth (i) (input_l) (0)))) (PreH12 : (INT_MIN <= current)) (PreH13 : (current <= INT_MAX)) (PreH14 : (special_filter_prefix_146 input_l i num )) ,
+  ((( &( "last" ) )) # Int  |->_)
+  **  ((( &( "first" ) )) # Int  |-> current)
+  **  ((( &( "nums" ) )) # Ptr  |-> nums_pre)
+  **  ((( &( "nums_size" ) )) # Int  |-> nums_size_pre)
+  **  ((( &( "i" ) )) # Int  |-> i)
+  **  ((( &( "num" ) )) # Int  |-> num)
+  **  ((( &( "current" ) )) # Int  |-> current)
+  **  (IntArray.full nums_pre nums_size_pre input_l )
+|--
+  “ (10 <= INT_MAX) ” 
+  &&  “ ((INT_MIN) <= 10) ”
+.
+
+Definition specialFilter_safety_wit_6 := 
+forall (nums_size_pre: Z) (nums_pre: Z) (input_l: (@list Z)) (last: Z) (first: Z) (current: Z) (num: Z) (i: Z) (PreH1 : (0 <= nums_size_pre)) (PreH2 : (nums_size_pre < INT_MAX)) (PreH3 : (nums_size_pre = (Zlength (input_l)))) (PreH4 : (problem_146_pre_z input_l )) (PreH5 : (special_filter_safe_146 input_l )) (PreH6 : (0 <= i)) (PreH7 : (i < nums_size_pre)) (PreH8 : (0 <= num)) (PreH9 : (num <= i)) (PreH10 : (current = (Znth (i) (input_l) (0)))) (PreH11 : (current > 10)) (PreH12 : (INT_MIN <= current)) (PreH13 : (current <= INT_MAX)) (PreH14 : (1 <= first)) (PreH15 : (first <= current)) (PreH16 : (last = (current % ( 10 ) ))) (PreH17 : (first_digit_state_146 current first )) (PreH18 : (special_filter_prefix_146 input_l i num )) ,
+  ((( &( "nums" ) )) # Ptr  |-> nums_pre)
+  **  ((( &( "nums_size" ) )) # Int  |-> nums_size_pre)
+  **  ((( &( "i" ) )) # Int  |-> i)
+  **  ((( &( "num" ) )) # Int  |-> num)
+  **  ((( &( "current" ) )) # Int  |-> current)
+  **  ((( &( "first" ) )) # Int  |-> first)
+  **  ((( &( "last" ) )) # Int  |-> last)
+  **  (IntArray.full nums_pre nums_size_pre input_l )
+|--
+  “ (10 <= INT_MAX) ” 
+  &&  “ ((INT_MIN) <= 10) ”
+.
+
+Definition specialFilter_safety_wit_7 := 
+forall (nums_size_pre: Z) (nums_pre: Z) (input_l: (@list Z)) (last: Z) (first: Z) (current: Z) (num: Z) (i: Z) (PreH1 : (first >= 10)) (PreH2 : (0 <= nums_size_pre)) (PreH3 : (nums_size_pre < INT_MAX)) (PreH4 : (nums_size_pre = (Zlength (input_l)))) (PreH5 : (problem_146_pre_z input_l )) (PreH6 : (special_filter_safe_146 input_l )) (PreH7 : (0 <= i)) (PreH8 : (i < nums_size_pre)) (PreH9 : (0 <= num)) (PreH10 : (num <= i)) (PreH11 : (current = (Znth (i) (input_l) (0)))) (PreH12 : (current > 10)) (PreH13 : (INT_MIN <= current)) (PreH14 : (current <= INT_MAX)) (PreH15 : (1 <= first)) (PreH16 : (first <= current)) (PreH17 : (last = (current % ( 10 ) ))) (PreH18 : (first_digit_state_146 current first )) (PreH19 : (special_filter_prefix_146 input_l i num )) ,
+  ((( &( "nums" ) )) # Ptr  |-> nums_pre)
+  **  ((( &( "nums_size" ) )) # Int  |-> nums_size_pre)
+  **  ((( &( "i" ) )) # Int  |-> i)
+  **  ((( &( "num" ) )) # Int  |-> num)
+  **  ((( &( "current" ) )) # Int  |-> current)
+  **  ((( &( "first" ) )) # Int  |-> first)
+  **  ((( &( "last" ) )) # Int  |-> last)
+  **  (IntArray.full nums_pre nums_size_pre input_l )
+|--
+  “ ((first <> (INT_MIN)) \/ (10 <> (-1))) ” 
+  &&  “ (10 <> 0) ”
+.
+
+Definition specialFilter_safety_wit_8 := 
+forall (nums_size_pre: Z) (nums_pre: Z) (input_l: (@list Z)) (last: Z) (first: Z) (current: Z) (num: Z) (i: Z) (PreH1 : (first >= 10)) (PreH2 : (0 <= nums_size_pre)) (PreH3 : (nums_size_pre < INT_MAX)) (PreH4 : (nums_size_pre = (Zlength (input_l)))) (PreH5 : (problem_146_pre_z input_l )) (PreH6 : (special_filter_safe_146 input_l )) (PreH7 : (0 <= i)) (PreH8 : (i < nums_size_pre)) (PreH9 : (0 <= num)) (PreH10 : (num <= i)) (PreH11 : (current = (Znth (i) (input_l) (0)))) (PreH12 : (current > 10)) (PreH13 : (INT_MIN <= current)) (PreH14 : (current <= INT_MAX)) (PreH15 : (1 <= first)) (PreH16 : (first <= current)) (PreH17 : (last = (current % ( 10 ) ))) (PreH18 : (first_digit_state_146 current first )) (PreH19 : (special_filter_prefix_146 input_l i num )) ,
+  ((( &( "nums" ) )) # Ptr  |-> nums_pre)
+  **  ((( &( "nums_size" ) )) # Int  |-> nums_size_pre)
+  **  ((( &( "i" ) )) # Int  |-> i)
+  **  ((( &( "num" ) )) # Int  |-> num)
+  **  ((( &( "current" ) )) # Int  |-> current)
+  **  ((( &( "first" ) )) # Int  |-> first)
+  **  ((( &( "last" ) )) # Int  |-> last)
+  **  (IntArray.full nums_pre nums_size_pre input_l )
+|--
+  “ (10 <= INT_MAX) ” 
+  &&  “ ((INT_MIN) <= 10) ”
+.
+
+Definition specialFilter_safety_wit_9 := 
+forall (nums_size_pre: Z) (nums_pre: Z) (input_l: (@list Z)) (i: Z) (num: Z) (current: Z) (first: Z) (last: Z) (PreH1 : (0 <= nums_size_pre)) (PreH2 : (nums_size_pre < INT_MAX)) (PreH3 : (nums_size_pre = (Zlength (input_l)))) (PreH4 : (problem_146_pre_z input_l )) (PreH5 : (special_filter_safe_146 input_l )) (PreH6 : (0 <= i)) (PreH7 : (i < nums_size_pre)) (PreH8 : (0 <= num)) (PreH9 : (num <= i)) (PreH10 : (current = (Znth (i) (input_l) (0)))) (PreH11 : (current > 10)) (PreH12 : (INT_MIN <= current)) (PreH13 : (current <= INT_MAX)) (PreH14 : (1 <= first)) (PreH15 : (first < 10)) (PreH16 : (last = (current % ( 10 ) ))) (PreH17 : (first_digit_state_146 current first )) (PreH18 : (special_filter_prefix_146 input_l i num )) ,
+  ((( &( "nums" ) )) # Ptr  |-> nums_pre)
+  **  ((( &( "nums_size" ) )) # Int  |-> nums_size_pre)
+  **  ((( &( "i" ) )) # Int  |-> i)
+  **  ((( &( "num" ) )) # Int  |-> num)
+  **  ((( &( "current" ) )) # Int  |-> current)
+  **  ((( &( "first" ) )) # Int  |-> first)
+  **  ((( &( "last" ) )) # Int  |-> last)
+  **  (IntArray.full nums_pre nums_size_pre input_l )
+|--
+  “ ((first <> (INT_MIN)) \/ (2 <> (-1))) ” 
+  &&  “ (2 <> 0) ”
+.
+
+Definition specialFilter_safety_wit_10 := 
+forall (nums_size_pre: Z) (nums_pre: Z) (input_l: (@list Z)) (i: Z) (num: Z) (current: Z) (first: Z) (last: Z) (PreH1 : (0 <= nums_size_pre)) (PreH2 : (nums_size_pre < INT_MAX)) (PreH3 : (nums_size_pre = (Zlength (input_l)))) (PreH4 : (problem_146_pre_z input_l )) (PreH5 : (special_filter_safe_146 input_l )) (PreH6 : (0 <= i)) (PreH7 : (i < nums_size_pre)) (PreH8 : (0 <= num)) (PreH9 : (num <= i)) (PreH10 : (current = (Znth (i) (input_l) (0)))) (PreH11 : (current > 10)) (PreH12 : (INT_MIN <= current)) (PreH13 : (current <= INT_MAX)) (PreH14 : (1 <= first)) (PreH15 : (first < 10)) (PreH16 : (last = (current % ( 10 ) ))) (PreH17 : (first_digit_state_146 current first )) (PreH18 : (special_filter_prefix_146 input_l i num )) ,
+  ((( &( "nums" ) )) # Ptr  |-> nums_pre)
+  **  ((( &( "nums_size" ) )) # Int  |-> nums_size_pre)
+  **  ((( &( "i" ) )) # Int  |-> i)
+  **  ((( &( "num" ) )) # Int  |-> num)
+  **  ((( &( "current" ) )) # Int  |-> current)
+  **  ((( &( "first" ) )) # Int  |-> first)
+  **  ((( &( "last" ) )) # Int  |-> last)
+  **  (IntArray.full nums_pre nums_size_pre input_l )
+|--
+  “ (2 <= INT_MAX) ” 
+  &&  “ ((INT_MIN) <= 2) ”
+.
+
+Definition specialFilter_safety_wit_11 := 
+forall (nums_size_pre: Z) (nums_pre: Z) (input_l: (@list Z)) (i: Z) (num: Z) (current: Z) (first: Z) (last: Z) (PreH1 : (0 <= nums_size_pre)) (PreH2 : (nums_size_pre < INT_MAX)) (PreH3 : (nums_size_pre = (Zlength (input_l)))) (PreH4 : (problem_146_pre_z input_l )) (PreH5 : (special_filter_safe_146 input_l )) (PreH6 : (0 <= i)) (PreH7 : (i < nums_size_pre)) (PreH8 : (0 <= num)) (PreH9 : (num <= i)) (PreH10 : (current = (Znth (i) (input_l) (0)))) (PreH11 : (current > 10)) (PreH12 : (INT_MIN <= current)) (PreH13 : (current <= INT_MAX)) (PreH14 : (1 <= first)) (PreH15 : (first < 10)) (PreH16 : (last = (current % ( 10 ) ))) (PreH17 : (first_digit_state_146 current first )) (PreH18 : (special_filter_prefix_146 input_l i num )) ,
+  ((( &( "nums" ) )) # Ptr  |-> nums_pre)
+  **  ((( &( "nums_size" ) )) # Int  |-> nums_size_pre)
+  **  ((( &( "i" ) )) # Int  |-> i)
+  **  ((( &( "num" ) )) # Int  |-> num)
+  **  ((( &( "current" ) )) # Int  |-> current)
+  **  ((( &( "first" ) )) # Int  |-> first)
+  **  ((( &( "last" ) )) # Int  |-> last)
+  **  (IntArray.full nums_pre nums_size_pre input_l )
+|--
+  “ (1 <= INT_MAX) ” 
+  &&  “ ((INT_MIN) <= 1) ”
+.
+
+Definition specialFilter_safety_wit_12 := 
+forall (nums_size_pre: Z) (nums_pre: Z) (input_l: (@list Z)) (i: Z) (num: Z) (current: Z) (first: Z) (last: Z) (PreH1 : ((first % ( 2 ) ) = 1)) (PreH2 : (0 <= nums_size_pre)) (PreH3 : (nums_size_pre < INT_MAX)) (PreH4 : (nums_size_pre = (Zlength (input_l)))) (PreH5 : (problem_146_pre_z input_l )) (PreH6 : (special_filter_safe_146 input_l )) (PreH7 : (0 <= i)) (PreH8 : (i < nums_size_pre)) (PreH9 : (0 <= num)) (PreH10 : (num <= i)) (PreH11 : (current = (Znth (i) (input_l) (0)))) (PreH12 : (current > 10)) (PreH13 : (INT_MIN <= current)) (PreH14 : (current <= INT_MAX)) (PreH15 : (1 <= first)) (PreH16 : (first < 10)) (PreH17 : (last = (current % ( 10 ) ))) (PreH18 : (first_digit_state_146 current first )) (PreH19 : (special_filter_prefix_146 input_l i num )) ,
+  ((( &( "nums" ) )) # Ptr  |-> nums_pre)
+  **  ((( &( "nums_size" ) )) # Int  |-> nums_size_pre)
+  **  ((( &( "i" ) )) # Int  |-> i)
+  **  ((( &( "num" ) )) # Int  |-> num)
+  **  ((( &( "current" ) )) # Int  |-> current)
+  **  ((( &( "first" ) )) # Int  |-> first)
+  **  ((( &( "last" ) )) # Int  |-> last)
+  **  (IntArray.full nums_pre nums_size_pre input_l )
+|--
+  “ ((last <> (INT_MIN)) \/ (2 <> (-1))) ” 
+  &&  “ (2 <> 0) ”
+.
+
+Definition specialFilter_safety_wit_13 := 
+forall (nums_size_pre: Z) (nums_pre: Z) (input_l: (@list Z)) (i: Z) (num: Z) (current: Z) (first: Z) (last: Z) (PreH1 : ((first % ( 2 ) ) = 1)) (PreH2 : (0 <= nums_size_pre)) (PreH3 : (nums_size_pre < INT_MAX)) (PreH4 : (nums_size_pre = (Zlength (input_l)))) (PreH5 : (problem_146_pre_z input_l )) (PreH6 : (special_filter_safe_146 input_l )) (PreH7 : (0 <= i)) (PreH8 : (i < nums_size_pre)) (PreH9 : (0 <= num)) (PreH10 : (num <= i)) (PreH11 : (current = (Znth (i) (input_l) (0)))) (PreH12 : (current > 10)) (PreH13 : (INT_MIN <= current)) (PreH14 : (current <= INT_MAX)) (PreH15 : (1 <= first)) (PreH16 : (first < 10)) (PreH17 : (last = (current % ( 10 ) ))) (PreH18 : (first_digit_state_146 current first )) (PreH19 : (special_filter_prefix_146 input_l i num )) ,
+  ((( &( "nums" ) )) # Ptr  |-> nums_pre)
+  **  ((( &( "nums_size" ) )) # Int  |-> nums_size_pre)
+  **  ((( &( "i" ) )) # Int  |-> i)
+  **  ((( &( "num" ) )) # Int  |-> num)
+  **  ((( &( "current" ) )) # Int  |-> current)
+  **  ((( &( "first" ) )) # Int  |-> first)
+  **  ((( &( "last" ) )) # Int  |-> last)
+  **  (IntArray.full nums_pre nums_size_pre input_l )
+|--
+  “ (2 <= INT_MAX) ” 
+  &&  “ ((INT_MIN) <= 2) ”
+.
+
+Definition specialFilter_safety_wit_14 := 
+forall (nums_size_pre: Z) (nums_pre: Z) (input_l: (@list Z)) (i: Z) (num: Z) (current: Z) (first: Z) (last: Z) (PreH1 : ((first % ( 2 ) ) = 1)) (PreH2 : (0 <= nums_size_pre)) (PreH3 : (nums_size_pre < INT_MAX)) (PreH4 : (nums_size_pre = (Zlength (input_l)))) (PreH5 : (problem_146_pre_z input_l )) (PreH6 : (special_filter_safe_146 input_l )) (PreH7 : (0 <= i)) (PreH8 : (i < nums_size_pre)) (PreH9 : (0 <= num)) (PreH10 : (num <= i)) (PreH11 : (current = (Znth (i) (input_l) (0)))) (PreH12 : (current > 10)) (PreH13 : (INT_MIN <= current)) (PreH14 : (current <= INT_MAX)) (PreH15 : (1 <= first)) (PreH16 : (first < 10)) (PreH17 : (last = (current % ( 10 ) ))) (PreH18 : (first_digit_state_146 current first )) (PreH19 : (special_filter_prefix_146 input_l i num )) ,
+  ((( &( "nums" ) )) # Ptr  |-> nums_pre)
+  **  ((( &( "nums_size" ) )) # Int  |-> nums_size_pre)
+  **  ((( &( "i" ) )) # Int  |-> i)
+  **  ((( &( "num" ) )) # Int  |-> num)
+  **  ((( &( "current" ) )) # Int  |-> current)
+  **  ((( &( "first" ) )) # Int  |-> first)
+  **  ((( &( "last" ) )) # Int  |-> last)
+  **  (IntArray.full nums_pre nums_size_pre input_l )
+|--
+  “ (1 <= INT_MAX) ” 
+  &&  “ ((INT_MIN) <= 1) ”
+.
+
+Definition specialFilter_safety_wit_15 := 
+forall (nums_size_pre: Z) (nums_pre: Z) (input_l: (@list Z)) (i: Z) (num: Z) (current: Z) (first: Z) (last: Z) (PreH1 : ((last % ( 2 ) ) = 1)) (PreH2 : ((first % ( 2 ) ) = 1)) (PreH3 : (0 <= nums_size_pre)) (PreH4 : (nums_size_pre < INT_MAX)) (PreH5 : (nums_size_pre = (Zlength (input_l)))) (PreH6 : (problem_146_pre_z input_l )) (PreH7 : (special_filter_safe_146 input_l )) (PreH8 : (0 <= i)) (PreH9 : (i < nums_size_pre)) (PreH10 : (0 <= num)) (PreH11 : (num <= i)) (PreH12 : (current = (Znth (i) (input_l) (0)))) (PreH13 : (current > 10)) (PreH14 : (INT_MIN <= current)) (PreH15 : (current <= INT_MAX)) (PreH16 : (1 <= first)) (PreH17 : (first < 10)) (PreH18 : (last = (current % ( 10 ) ))) (PreH19 : (first_digit_state_146 current first )) (PreH20 : (special_filter_prefix_146 input_l i num )) ,
+  ((( &( "nums" ) )) # Ptr  |-> nums_pre)
+  **  ((( &( "nums_size" ) )) # Int  |-> nums_size_pre)
+  **  ((( &( "i" ) )) # Int  |-> i)
+  **  ((( &( "num" ) )) # Int  |-> num)
+  **  ((( &( "current" ) )) # Int  |-> current)
+  **  ((( &( "first" ) )) # Int  |-> first)
+  **  ((( &( "last" ) )) # Int  |-> last)
+  **  (IntArray.full nums_pre nums_size_pre input_l )
+|--
+  “ ((num + 1 ) <= INT_MAX) ” 
+  &&  “ ((INT_MIN) <= (num + 1 )) ”
+.
+
+Definition specialFilter_safety_wit_16 := 
+forall (nums_size_pre: Z) (nums_pre: Z) (input_l: (@list Z)) (i: Z) (num: Z) (current: Z) (first: Z) (last: Z) (PreH1 : ((last % ( 2 ) ) = 1)) (PreH2 : ((first % ( 2 ) ) = 1)) (PreH3 : (0 <= nums_size_pre)) (PreH4 : (nums_size_pre < INT_MAX)) (PreH5 : (nums_size_pre = (Zlength (input_l)))) (PreH6 : (problem_146_pre_z input_l )) (PreH7 : (special_filter_safe_146 input_l )) (PreH8 : (0 <= i)) (PreH9 : (i < nums_size_pre)) (PreH10 : (0 <= num)) (PreH11 : (num <= i)) (PreH12 : (current = (Znth (i) (input_l) (0)))) (PreH13 : (current > 10)) (PreH14 : (INT_MIN <= current)) (PreH15 : (current <= INT_MAX)) (PreH16 : (1 <= first)) (PreH17 : (first < 10)) (PreH18 : (last = (current % ( 10 ) ))) (PreH19 : (first_digit_state_146 current first )) (PreH20 : (special_filter_prefix_146 input_l i num )) ,
+  ((( &( "nums" ) )) # Ptr  |-> nums_pre)
+  **  ((( &( "nums_size" ) )) # Int  |-> nums_size_pre)
+  **  ((( &( "i" ) )) # Int  |-> i)
+  **  ((( &( "num" ) )) # Int  |-> num)
+  **  ((( &( "current" ) )) # Int  |-> current)
+  **  ((( &( "first" ) )) # Int  |-> first)
+  **  ((( &( "last" ) )) # Int  |-> last)
+  **  (IntArray.full nums_pre nums_size_pre input_l )
+|--
+  “ (1 <= INT_MAX) ” 
+  &&  “ ((INT_MIN) <= 1) ”
+.
+
+Definition specialFilter_safety_wit_17 := 
+forall (nums_size_pre: Z) (nums_pre: Z) (input_l: (@list Z)) (i: Z) (num: Z) (current: Z) (first: Z) (last: Z) (PreH1 : (0 <= nums_size_pre)) (PreH2 : (nums_size_pre < INT_MAX)) (PreH3 : (nums_size_pre = (Zlength (input_l)))) (PreH4 : (problem_146_pre_z input_l )) (PreH5 : (special_filter_safe_146 input_l )) (PreH6 : (0 <= i)) (PreH7 : (i < nums_size_pre)) (PreH8 : (0 <= num)) (PreH9 : (num <= (i + 1 ))) (PreH10 : (current = (Znth (i) (input_l) (0)))) (PreH11 : (current > 10)) (PreH12 : (first_digit_state_146 current first )) (PreH13 : (first < 10)) (PreH14 : (last = (current % ( 10 ) ))) (PreH15 : ((first % ( 2 ) ) = 1)) (PreH16 : ((last % ( 2 ) ) = 1)) (PreH17 : (special_filter_prefix_146 input_l (i + 1 ) num )) ,
+  ((( &( "nums" ) )) # Ptr  |-> nums_pre)
+  **  ((( &( "nums_size" ) )) # Int  |-> nums_size_pre)
+  **  ((( &( "i" ) )) # Int  |-> i)
+  **  ((( &( "num" ) )) # Int  |-> num)
+  **  (IntArray.full nums_pre nums_size_pre input_l )
+|--
+  “ ((i + 1 ) <= INT_MAX) ” 
+  &&  “ ((INT_MIN) <= (i + 1 )) ”
+.
+
+Definition specialFilter_safety_wit_18 := 
+forall (nums_size_pre: Z) (nums_pre: Z) (input_l: (@list Z)) (i: Z) (num: Z) (current: Z) (first: Z) (last: Z) (PreH1 : (0 <= nums_size_pre)) (PreH2 : (nums_size_pre < INT_MAX)) (PreH3 : (nums_size_pre = (Zlength (input_l)))) (PreH4 : (problem_146_pre_z input_l )) (PreH5 : (special_filter_safe_146 input_l )) (PreH6 : (0 <= i)) (PreH7 : (i < nums_size_pre)) (PreH8 : (0 <= num)) (PreH9 : (num <= i)) (PreH10 : (current = (Znth (i) (input_l) (0)))) (PreH11 : (current > 10)) (PreH12 : (first_digit_state_146 current first )) (PreH13 : (first < 10)) (PreH14 : (last = (current % ( 10 ) ))) (PreH15 : ((last % ( 2 ) ) <> 1)) (PreH16 : (special_filter_prefix_146 input_l (i + 1 ) num )) ,
+  ((( &( "nums" ) )) # Ptr  |-> nums_pre)
+  **  ((( &( "nums_size" ) )) # Int  |-> nums_size_pre)
+  **  ((( &( "i" ) )) # Int  |-> i)
+  **  ((( &( "num" ) )) # Int  |-> num)
+  **  (IntArray.full nums_pre nums_size_pre input_l )
+|--
+  “ ((i + 1 ) <= INT_MAX) ” 
+  &&  “ ((INT_MIN) <= (i + 1 )) ”
+.
+
+Definition specialFilter_safety_wit_19 := 
+forall (nums_size_pre: Z) (nums_pre: Z) (input_l: (@list Z)) (i: Z) (num: Z) (current: Z) (first: Z) (last: Z) (PreH1 : (0 <= nums_size_pre)) (PreH2 : (nums_size_pre < INT_MAX)) (PreH3 : (nums_size_pre = (Zlength (input_l)))) (PreH4 : (problem_146_pre_z input_l )) (PreH5 : (special_filter_safe_146 input_l )) (PreH6 : (0 <= i)) (PreH7 : (i < nums_size_pre)) (PreH8 : (0 <= num)) (PreH9 : (num <= i)) (PreH10 : (current = (Znth (i) (input_l) (0)))) (PreH11 : (current > 10)) (PreH12 : (first_digit_state_146 current first )) (PreH13 : (first < 10)) (PreH14 : (last = (current % ( 10 ) ))) (PreH15 : ((first % ( 2 ) ) <> 1)) (PreH16 : (special_filter_prefix_146 input_l (i + 1 ) num )) ,
+  ((( &( "nums" ) )) # Ptr  |-> nums_pre)
+  **  ((( &( "nums_size" ) )) # Int  |-> nums_size_pre)
+  **  ((( &( "i" ) )) # Int  |-> i)
+  **  ((( &( "num" ) )) # Int  |-> num)
+  **  (IntArray.full nums_pre nums_size_pre input_l )
+|--
+  “ ((i + 1 ) <= INT_MAX) ” 
+  &&  “ ((INT_MIN) <= (i + 1 )) ”
+.
+
+Definition specialFilter_safety_wit_20 := 
+forall (nums_size_pre: Z) (nums_pre: Z) (input_l: (@list Z)) (i: Z) (num: Z) (current: Z) (PreH1 : (0 <= nums_size_pre)) (PreH2 : (nums_size_pre < INT_MAX)) (PreH3 : (nums_size_pre = (Zlength (input_l)))) (PreH4 : (problem_146_pre_z input_l )) (PreH5 : (special_filter_safe_146 input_l )) (PreH6 : (0 <= i)) (PreH7 : (i < nums_size_pre)) (PreH8 : (0 <= num)) (PreH9 : (num <= i)) (PreH10 : (current = (Znth (i) (input_l) (0)))) (PreH11 : (current <= 10)) (PreH12 : (special_filter_prefix_146 input_l (i + 1 ) num )) ,
+  ((( &( "nums" ) )) # Ptr  |-> nums_pre)
+  **  ((( &( "nums_size" ) )) # Int  |-> nums_size_pre)
+  **  ((( &( "i" ) )) # Int  |-> i)
+  **  ((( &( "num" ) )) # Int  |-> num)
+  **  (IntArray.full nums_pre nums_size_pre input_l )
+|--
+  “ ((i + 1 ) <= INT_MAX) ” 
+  &&  “ ((INT_MIN) <= (i + 1 )) ”
+.
+
+Definition specialFilter_entail_wit_1 := 
+(
+forall (nums_size_pre: Z) (nums_pre: Z) (input_l: (@list Z)) (PreH1 : (nums_pre <> 0)) (PreH2 : (0 <= nums_size_pre)) (PreH3 : (nums_size_pre < INT_MAX)) (PreH4 : (nums_size_pre = (Zlength (input_l)))) (PreH5 : (problem_146_pre_z input_l )) (PreH6 : (special_filter_safe_146 input_l )) ,
+  (IntArray.full nums_pre nums_size_pre input_l )
+|--
+  “ (0 <= nums_size_pre) ” 
+  &&  “ (nums_size_pre < INT_MAX) ” 
+  &&  “ (nums_size_pre = (Zlength (input_l))) ” 
+  &&  “ (problem_146_pre_z input_l ) ” 
+  &&  “ (special_filter_safe_146 input_l ) ” 
+  &&  “ (0 <= 0) ” 
+  &&  “ (0 <= nums_size_pre) ” 
+  &&  “ (0 <= 0) ” 
+  &&  “ (0 <= 0) ” 
+  &&  “ (special_filter_prefix_146 input_l 0 0 ) ”
+  &&  (IntArray.full nums_pre nums_size_pre input_l )
+) \/
+(
+forall (nums_size_pre: Z) (nums_pre: Z) (input_l: (@list Z)) (PreH1 : (nums_pre <> 0)) (PreH2 : (0 <= nums_size_pre)) (PreH3 : (nums_size_pre < INT_MAX)) (PreH4 : (nums_size_pre = (Zlength (input_l)))) (PreH5 : (problem_146_pre_z input_l )) (PreH6 : (special_filter_safe_146 input_l )) ,
+  TT && emp 
+|--
+  “ (special_filter_prefix_146 input_l 0 0 ) ”
+  &&  emp
+).
+
+Definition specialFilter_entail_wit_1_split_goal_1 := 
+forall (nums_size_pre: Z) (nums_pre: Z) (input_l: (@list Z)) (PreH1 : (nums_pre <> 0)) (PreH2 : (0 <= nums_size_pre)) (PreH3 : (nums_size_pre < INT_MAX)) (PreH4 : (nums_size_pre = (Zlength (input_l)))) (PreH5 : (problem_146_pre_z input_l )) (PreH6 : (special_filter_safe_146 input_l )) ,
+  TT && emp 
+|--
+  “ (special_filter_prefix_146 input_l 0 0 ) ”
+.
+
+Definition specialFilter_entail_wit_2 := 
+(
+forall (nums_size_pre: Z) (nums_pre: Z) (input_l: (@list Z)) (num: Z) (i: Z) (PreH1 : (i < nums_size_pre)) (PreH2 : (0 <= nums_size_pre)) (PreH3 : (nums_size_pre < INT_MAX)) (PreH4 : (nums_size_pre = (Zlength (input_l)))) (PreH5 : (problem_146_pre_z input_l )) (PreH6 : (special_filter_safe_146 input_l )) (PreH7 : (0 <= i)) (PreH8 : (i <= nums_size_pre)) (PreH9 : (0 <= num)) (PreH10 : (num <= i)) (PreH11 : (special_filter_prefix_146 input_l i num )) ,
+  (IntArray.full nums_pre nums_size_pre input_l )
+|--
+  “ (0 <= nums_size_pre) ” 
+  &&  “ (nums_size_pre < INT_MAX) ” 
+  &&  “ (nums_size_pre = (Zlength (input_l))) ” 
+  &&  “ (problem_146_pre_z input_l ) ” 
+  &&  “ (special_filter_safe_146 input_l ) ” 
+  &&  “ (0 <= i) ” 
+  &&  “ (i < nums_size_pre) ” 
+  &&  “ (0 <= num) ” 
+  &&  “ (num <= i) ” 
+  &&  “ ((Znth i input_l 0) = (Znth (i) (input_l) (0))) ” 
+  &&  “ (INT_MIN <= (Znth i input_l 0)) ” 
+  &&  “ ((Znth i input_l 0) <= INT_MAX) ” 
+  &&  “ (special_filter_prefix_146 input_l i num ) ”
+  &&  (IntArray.full nums_pre nums_size_pre input_l )
+) \/
+(
+forall (nums_size_pre: Z) (input_l: (@list Z)) (num: Z) (i: Z) (PreH1 : (i < nums_size_pre)) (PreH2 : (0 <= nums_size_pre)) (PreH3 : (nums_size_pre < INT_MAX)) (PreH4 : (nums_size_pre = (Zlength (input_l)))) (PreH5 : (problem_146_pre_z input_l )) (PreH6 : (special_filter_safe_146 input_l )) (PreH7 : (0 <= i)) (PreH8 : (i <= nums_size_pre)) (PreH9 : (0 <= num)) (PreH10 : (num <= i)) (PreH11 : (special_filter_prefix_146 input_l i num )) ,
+  TT && emp 
+|--
+  “ ((Znth i input_l 0) <= INT_MAX) ” 
+  &&  “ (INT_MIN <= (Znth i input_l 0)) ” 
+  &&  “ ((Znth i input_l 0) = (Znth (i) (input_l) (0))) ”
+  &&  emp
+).
+
+Definition specialFilter_entail_wit_2_split_goal_1 := 
+forall (nums_size_pre: Z) (input_l: (@list Z)) (num: Z) (i: Z) (PreH1 : (i < nums_size_pre)) (PreH2 : (0 <= nums_size_pre)) (PreH3 : (nums_size_pre < INT_MAX)) (PreH4 : (nums_size_pre = (Zlength (input_l)))) (PreH5 : (problem_146_pre_z input_l )) (PreH6 : (special_filter_safe_146 input_l )) (PreH7 : (0 <= i)) (PreH8 : (i <= nums_size_pre)) (PreH9 : (0 <= num)) (PreH10 : (num <= i)) (PreH11 : (special_filter_prefix_146 input_l i num )) ,
+  TT && emp 
+|--
+  “ ((Znth i input_l 0) <= INT_MAX) ”
+.
+
+Definition specialFilter_entail_wit_2_split_goal_2 := 
+forall (nums_size_pre: Z) (input_l: (@list Z)) (num: Z) (i: Z) (PreH1 : (i < nums_size_pre)) (PreH2 : (0 <= nums_size_pre)) (PreH3 : (nums_size_pre < INT_MAX)) (PreH4 : (nums_size_pre = (Zlength (input_l)))) (PreH5 : (problem_146_pre_z input_l )) (PreH6 : (special_filter_safe_146 input_l )) (PreH7 : (0 <= i)) (PreH8 : (i <= nums_size_pre)) (PreH9 : (0 <= num)) (PreH10 : (num <= i)) (PreH11 : (special_filter_prefix_146 input_l i num )) ,
+  TT && emp 
+|--
+  “ (INT_MIN <= (Znth i input_l 0)) ”
+.
+
+Definition specialFilter_entail_wit_2_split_goal_3 := 
+forall (nums_size_pre: Z) (input_l: (@list Z)) (num: Z) (i: Z) (PreH1 : (i < nums_size_pre)) (PreH2 : (0 <= nums_size_pre)) (PreH3 : (nums_size_pre < INT_MAX)) (PreH4 : (nums_size_pre = (Zlength (input_l)))) (PreH5 : (problem_146_pre_z input_l )) (PreH6 : (special_filter_safe_146 input_l )) (PreH7 : (0 <= i)) (PreH8 : (i <= nums_size_pre)) (PreH9 : (0 <= num)) (PreH10 : (num <= i)) (PreH11 : (special_filter_prefix_146 input_l i num )) ,
+  TT && emp 
+|--
+  “ ((Znth i input_l 0) = (Znth (i) (input_l) (0))) ”
+.
+
+Definition specialFilter_entail_wit_3 := 
+(
+forall (nums_size_pre: Z) (nums_pre: Z) (input_l: (@list Z)) (i: Z) (num: Z) (current: Z) (PreH1 : (current > 10)) (PreH2 : (0 <= nums_size_pre)) (PreH3 : (nums_size_pre < INT_MAX)) (PreH4 : (nums_size_pre = (Zlength (input_l)))) (PreH5 : (problem_146_pre_z input_l )) (PreH6 : (special_filter_safe_146 input_l )) (PreH7 : (0 <= i)) (PreH8 : (i < nums_size_pre)) (PreH9 : (0 <= num)) (PreH10 : (num <= i)) (PreH11 : (current = (Znth (i) (input_l) (0)))) (PreH12 : (INT_MIN <= current)) (PreH13 : (current <= INT_MAX)) (PreH14 : (special_filter_prefix_146 input_l i num )) ,
+  (IntArray.full nums_pre nums_size_pre input_l )
+|--
+  “ (0 <= nums_size_pre) ” 
+  &&  “ (nums_size_pre < INT_MAX) ” 
+  &&  “ (nums_size_pre = (Zlength (input_l))) ” 
+  &&  “ (problem_146_pre_z input_l ) ” 
+  &&  “ (special_filter_safe_146 input_l ) ” 
+  &&  “ (0 <= i) ” 
+  &&  “ (i < nums_size_pre) ” 
+  &&  “ (0 <= num) ” 
+  &&  “ (num <= i) ” 
+  &&  “ (current = (Znth (i) (input_l) (0))) ” 
+  &&  “ (current > 10) ” 
+  &&  “ (INT_MIN <= current) ” 
+  &&  “ (current <= INT_MAX) ” 
+  &&  “ (current = current) ” 
+  &&  “ ((current % ( 10 ) ) = (current % ( 10 ) )) ” 
+  &&  “ (first_digit_state_146 current current ) ” 
+  &&  “ (special_filter_prefix_146 input_l i num ) ”
+  &&  (IntArray.full nums_pre nums_size_pre input_l )
+) \/
+(
+forall (nums_size_pre: Z) (input_l: (@list Z)) (i: Z) (num: Z) (current: Z) (PreH1 : (current > 10)) (PreH2 : (0 <= nums_size_pre)) (PreH3 : (nums_size_pre < INT_MAX)) (PreH4 : (nums_size_pre = (Zlength (input_l)))) (PreH5 : (problem_146_pre_z input_l )) (PreH6 : (special_filter_safe_146 input_l )) (PreH7 : (0 <= i)) (PreH8 : (i < nums_size_pre)) (PreH9 : (0 <= num)) (PreH10 : (num <= i)) (PreH11 : (current = (Znth (i) (input_l) (0)))) (PreH12 : (INT_MIN <= current)) (PreH13 : (current <= INT_MAX)) (PreH14 : (special_filter_prefix_146 input_l i num )) ,
+  TT && emp 
+|--
+  “ (first_digit_state_146 current current ) ”
+  &&  emp
+).
+
+Definition specialFilter_entail_wit_3_split_goal_1 := 
+forall (nums_size_pre: Z) (input_l: (@list Z)) (i: Z) (num: Z) (current: Z) (PreH1 : (current > 10)) (PreH2 : (0 <= nums_size_pre)) (PreH3 : (nums_size_pre < INT_MAX)) (PreH4 : (nums_size_pre = (Zlength (input_l)))) (PreH5 : (problem_146_pre_z input_l )) (PreH6 : (special_filter_safe_146 input_l )) (PreH7 : (0 <= i)) (PreH8 : (i < nums_size_pre)) (PreH9 : (0 <= num)) (PreH10 : (num <= i)) (PreH11 : (current = (Znth (i) (input_l) (0)))) (PreH12 : (INT_MIN <= current)) (PreH13 : (current <= INT_MAX)) (PreH14 : (special_filter_prefix_146 input_l i num )) ,
+  TT && emp 
+|--
+  “ (first_digit_state_146 current current ) ”
+.
+
+Definition specialFilter_entail_wit_4 := 
+forall (nums_size_pre: Z) (nums_pre: Z) (input_l: (@list Z)) (i: Z) (num: Z) (current: Z) (first: Z) (last: Z) (PreH1 : (0 <= nums_size_pre)) (PreH2 : (nums_size_pre < INT_MAX)) (PreH3 : (nums_size_pre = (Zlength (input_l)))) (PreH4 : (problem_146_pre_z input_l )) (PreH5 : (special_filter_safe_146 input_l )) (PreH6 : (0 <= i)) (PreH7 : (i < nums_size_pre)) (PreH8 : (0 <= num)) (PreH9 : (num <= i)) (PreH10 : (current = (Znth (i) (input_l) (0)))) (PreH11 : (current > 10)) (PreH12 : (INT_MIN <= current)) (PreH13 : (current <= INT_MAX)) (PreH14 : (first = current)) (PreH15 : (last = (current % ( 10 ) ))) (PreH16 : (first_digit_state_146 current first )) (PreH17 : (special_filter_prefix_146 input_l i num )) ,
+  (IntArray.full nums_pre nums_size_pre input_l )
+|--
+  “ (0 <= nums_size_pre) ” 
+  &&  “ (nums_size_pre < INT_MAX) ” 
+  &&  “ (nums_size_pre = (Zlength (input_l))) ” 
+  &&  “ (problem_146_pre_z input_l ) ” 
+  &&  “ (special_filter_safe_146 input_l ) ” 
+  &&  “ (0 <= i) ” 
+  &&  “ (i < nums_size_pre) ” 
+  &&  “ (0 <= num) ” 
+  &&  “ (num <= i) ” 
+  &&  “ (current = (Znth (i) (input_l) (0))) ” 
+  &&  “ (current > 10) ” 
+  &&  “ (INT_MIN <= current) ” 
+  &&  “ (current <= INT_MAX) ” 
+  &&  “ (1 <= first) ” 
+  &&  “ (first <= current) ” 
+  &&  “ (last = (current % ( 10 ) )) ” 
+  &&  “ (first_digit_state_146 current first ) ” 
+  &&  “ (special_filter_prefix_146 input_l i num ) ”
+  &&  (IntArray.full nums_pre nums_size_pre input_l )
+.
+
+Definition specialFilter_entail_wit_5 := 
+(
+forall (nums_size_pre: Z) (nums_pre: Z) (input_l: (@list Z)) (last: Z) (first: Z) (current: Z) (num: Z) (i: Z) (PreH1 : (first >= 10)) (PreH2 : (0 <= nums_size_pre)) (PreH3 : (nums_size_pre < INT_MAX)) (PreH4 : (nums_size_pre = (Zlength (input_l)))) (PreH5 : (problem_146_pre_z input_l )) (PreH6 : (special_filter_safe_146 input_l )) (PreH7 : (0 <= i)) (PreH8 : (i < nums_size_pre)) (PreH9 : (0 <= num)) (PreH10 : (num <= i)) (PreH11 : (current = (Znth (i) (input_l) (0)))) (PreH12 : (current > 10)) (PreH13 : (INT_MIN <= current)) (PreH14 : (current <= INT_MAX)) (PreH15 : (1 <= first)) (PreH16 : (first <= current)) (PreH17 : (last = (current % ( 10 ) ))) (PreH18 : (first_digit_state_146 current first )) (PreH19 : (special_filter_prefix_146 input_l i num )) ,
+  (IntArray.full nums_pre nums_size_pre input_l )
+|--
+  “ (0 <= nums_size_pre) ” 
+  &&  “ (nums_size_pre < INT_MAX) ” 
+  &&  “ (nums_size_pre = (Zlength (input_l))) ” 
+  &&  “ (problem_146_pre_z input_l ) ” 
+  &&  “ (special_filter_safe_146 input_l ) ” 
+  &&  “ (0 <= i) ” 
+  &&  “ (i < nums_size_pre) ” 
+  &&  “ (0 <= num) ” 
+  &&  “ (num <= i) ” 
+  &&  “ (current = (Znth (i) (input_l) (0))) ” 
+  &&  “ (current > 10) ” 
+  &&  “ (INT_MIN <= current) ” 
+  &&  “ (current <= INT_MAX) ” 
+  &&  “ (1 <= (first ÷ 10 )) ” 
+  &&  “ ((first ÷ 10 ) <= current) ” 
+  &&  “ (last = (current % ( 10 ) )) ” 
+  &&  “ (first_digit_state_146 current (first ÷ 10 ) ) ” 
+  &&  “ (special_filter_prefix_146 input_l i num ) ”
+  &&  (IntArray.full nums_pre nums_size_pre input_l )
+) \/
+(
+forall (nums_size_pre: Z) (input_l: (@list Z)) (last: Z) (first: Z) (current: Z) (num: Z) (i: Z) (PreH1 : (first >= 10)) (PreH2 : (0 <= nums_size_pre)) (PreH3 : (nums_size_pre < INT_MAX)) (PreH4 : (nums_size_pre = (Zlength (input_l)))) (PreH5 : (problem_146_pre_z input_l )) (PreH6 : (special_filter_safe_146 input_l )) (PreH7 : (0 <= i)) (PreH8 : (i < nums_size_pre)) (PreH9 : (0 <= num)) (PreH10 : (num <= i)) (PreH11 : (current = (Znth (i) (input_l) (0)))) (PreH12 : (current > 10)) (PreH13 : (INT_MIN <= current)) (PreH14 : (current <= INT_MAX)) (PreH15 : (1 <= first)) (PreH16 : (first <= current)) (PreH17 : (last = (current % ( 10 ) ))) (PreH18 : (first_digit_state_146 current first )) (PreH19 : (special_filter_prefix_146 input_l i num )) ,
+  TT && emp 
+|--
+  “ (first_digit_state_146 current (first ÷ 10 ) ) ” 
+  &&  “ ((first ÷ 10 ) <= current) ” 
+  &&  “ (1 <= (first ÷ 10 )) ”
+  &&  emp
+).
+
+Definition specialFilter_entail_wit_5_split_goal_1 := 
+forall (nums_size_pre: Z) (input_l: (@list Z)) (last: Z) (first: Z) (current: Z) (num: Z) (i: Z) (PreH1 : (first >= 10)) (PreH2 : (0 <= nums_size_pre)) (PreH3 : (nums_size_pre < INT_MAX)) (PreH4 : (nums_size_pre = (Zlength (input_l)))) (PreH5 : (problem_146_pre_z input_l )) (PreH6 : (special_filter_safe_146 input_l )) (PreH7 : (0 <= i)) (PreH8 : (i < nums_size_pre)) (PreH9 : (0 <= num)) (PreH10 : (num <= i)) (PreH11 : (current = (Znth (i) (input_l) (0)))) (PreH12 : (current > 10)) (PreH13 : (INT_MIN <= current)) (PreH14 : (current <= INT_MAX)) (PreH15 : (1 <= first)) (PreH16 : (first <= current)) (PreH17 : (last = (current % ( 10 ) ))) (PreH18 : (first_digit_state_146 current first )) (PreH19 : (special_filter_prefix_146 input_l i num )) ,
+  TT && emp 
+|--
+  “ (first_digit_state_146 current (first ÷ 10 ) ) ”
+.
+
+Definition specialFilter_entail_wit_5_split_goal_2 := 
+forall (nums_size_pre: Z) (input_l: (@list Z)) (last: Z) (first: Z) (current: Z) (num: Z) (i: Z) (PreH1 : (first >= 10)) (PreH2 : (0 <= nums_size_pre)) (PreH3 : (nums_size_pre < INT_MAX)) (PreH4 : (nums_size_pre = (Zlength (input_l)))) (PreH5 : (problem_146_pre_z input_l )) (PreH6 : (special_filter_safe_146 input_l )) (PreH7 : (0 <= i)) (PreH8 : (i < nums_size_pre)) (PreH9 : (0 <= num)) (PreH10 : (num <= i)) (PreH11 : (current = (Znth (i) (input_l) (0)))) (PreH12 : (current > 10)) (PreH13 : (INT_MIN <= current)) (PreH14 : (current <= INT_MAX)) (PreH15 : (1 <= first)) (PreH16 : (first <= current)) (PreH17 : (last = (current % ( 10 ) ))) (PreH18 : (first_digit_state_146 current first )) (PreH19 : (special_filter_prefix_146 input_l i num )) ,
+  TT && emp 
+|--
+  “ ((first ÷ 10 ) <= current) ”
+.
+
+Definition specialFilter_entail_wit_5_split_goal_3 := 
+forall (nums_size_pre: Z) (input_l: (@list Z)) (last: Z) (first: Z) (current: Z) (num: Z) (i: Z) (PreH1 : (first >= 10)) (PreH2 : (0 <= nums_size_pre)) (PreH3 : (nums_size_pre < INT_MAX)) (PreH4 : (nums_size_pre = (Zlength (input_l)))) (PreH5 : (problem_146_pre_z input_l )) (PreH6 : (special_filter_safe_146 input_l )) (PreH7 : (0 <= i)) (PreH8 : (i < nums_size_pre)) (PreH9 : (0 <= num)) (PreH10 : (num <= i)) (PreH11 : (current = (Znth (i) (input_l) (0)))) (PreH12 : (current > 10)) (PreH13 : (INT_MIN <= current)) (PreH14 : (current <= INT_MAX)) (PreH15 : (1 <= first)) (PreH16 : (first <= current)) (PreH17 : (last = (current % ( 10 ) ))) (PreH18 : (first_digit_state_146 current first )) (PreH19 : (special_filter_prefix_146 input_l i num )) ,
+  TT && emp 
+|--
+  “ (1 <= (first ÷ 10 )) ”
+.
+
+Definition specialFilter_entail_wit_6 := 
+forall (nums_size_pre: Z) (nums_pre: Z) (input_l: (@list Z)) (last: Z) (first: Z) (current: Z) (num: Z) (i: Z) (PreH1 : (first < 10)) (PreH2 : (0 <= nums_size_pre)) (PreH3 : (nums_size_pre < INT_MAX)) (PreH4 : (nums_size_pre = (Zlength (input_l)))) (PreH5 : (problem_146_pre_z input_l )) (PreH6 : (special_filter_safe_146 input_l )) (PreH7 : (0 <= i)) (PreH8 : (i < nums_size_pre)) (PreH9 : (0 <= num)) (PreH10 : (num <= i)) (PreH11 : (current = (Znth (i) (input_l) (0)))) (PreH12 : (current > 10)) (PreH13 : (INT_MIN <= current)) (PreH14 : (current <= INT_MAX)) (PreH15 : (1 <= first)) (PreH16 : (first <= current)) (PreH17 : (last = (current % ( 10 ) ))) (PreH18 : (first_digit_state_146 current first )) (PreH19 : (special_filter_prefix_146 input_l i num )) ,
+  (IntArray.full nums_pre nums_size_pre input_l )
+|--
+  “ (0 <= nums_size_pre) ” 
+  &&  “ (nums_size_pre < INT_MAX) ” 
+  &&  “ (nums_size_pre = (Zlength (input_l))) ” 
+  &&  “ (problem_146_pre_z input_l ) ” 
+  &&  “ (special_filter_safe_146 input_l ) ” 
+  &&  “ (0 <= i) ” 
+  &&  “ (i < nums_size_pre) ” 
+  &&  “ (0 <= num) ” 
+  &&  “ (num <= i) ” 
+  &&  “ (current = (Znth (i) (input_l) (0))) ” 
+  &&  “ (current > 10) ” 
+  &&  “ (INT_MIN <= current) ” 
+  &&  “ (current <= INT_MAX) ” 
+  &&  “ (1 <= first) ” 
+  &&  “ (first < 10) ” 
+  &&  “ (last = (current % ( 10 ) )) ” 
+  &&  “ (first_digit_state_146 current first ) ” 
+  &&  “ (special_filter_prefix_146 input_l i num ) ”
+  &&  (IntArray.full nums_pre nums_size_pre input_l )
+.
+
+Definition specialFilter_entail_wit_7 := 
+(
+forall (nums_size_pre: Z) (nums_pre: Z) (input_l: (@list Z)) (i: Z) (num: Z) (current: Z) (first: Z) (last: Z) (PreH1 : ((last % ( 2 ) ) = 1)) (PreH2 : ((first % ( 2 ) ) = 1)) (PreH3 : (0 <= nums_size_pre)) (PreH4 : (nums_size_pre < INT_MAX)) (PreH5 : (nums_size_pre = (Zlength (input_l)))) (PreH6 : (problem_146_pre_z input_l )) (PreH7 : (special_filter_safe_146 input_l )) (PreH8 : (0 <= i)) (PreH9 : (i < nums_size_pre)) (PreH10 : (0 <= num)) (PreH11 : (num <= i)) (PreH12 : (current = (Znth (i) (input_l) (0)))) (PreH13 : (current > 10)) (PreH14 : (INT_MIN <= current)) (PreH15 : (current <= INT_MAX)) (PreH16 : (1 <= first)) (PreH17 : (first < 10)) (PreH18 : (last = (current % ( 10 ) ))) (PreH19 : (first_digit_state_146 current first )) (PreH20 : (special_filter_prefix_146 input_l i num )) ,
+  (IntArray.full nums_pre nums_size_pre input_l )
+|--
+  “ (0 <= nums_size_pre) ” 
+  &&  “ (nums_size_pre < INT_MAX) ” 
+  &&  “ (nums_size_pre = (Zlength (input_l))) ” 
+  &&  “ (problem_146_pre_z input_l ) ” 
+  &&  “ (special_filter_safe_146 input_l ) ” 
+  &&  “ (0 <= i) ” 
+  &&  “ (i < nums_size_pre) ” 
+  &&  “ (0 <= (num + 1 )) ” 
+  &&  “ ((num + 1 ) <= (i + 1 )) ” 
+  &&  “ (current = (Znth (i) (input_l) (0))) ” 
+  &&  “ (current > 10) ” 
+  &&  “ (first_digit_state_146 current first ) ” 
+  &&  “ (first < 10) ” 
+  &&  “ (last = (current % ( 10 ) )) ” 
+  &&  “ ((first % ( 2 ) ) = 1) ” 
+  &&  “ ((last % ( 2 ) ) = 1) ” 
+  &&  “ (special_filter_prefix_146 input_l (i + 1 ) (num + 1 ) ) ”
+  &&  (IntArray.full nums_pre nums_size_pre input_l )
+) \/
+(
+forall (nums_size_pre: Z) (input_l: (@list Z)) (i: Z) (num: Z) (current: Z) (first: Z) (last: Z) (PreH1 : ((last % ( 2 ) ) = 1)) (PreH2 : ((first % ( 2 ) ) = 1)) (PreH3 : (0 <= nums_size_pre)) (PreH4 : (nums_size_pre < INT_MAX)) (PreH5 : (nums_size_pre = (Zlength (input_l)))) (PreH6 : (problem_146_pre_z input_l )) (PreH7 : (special_filter_safe_146 input_l )) (PreH8 : (0 <= i)) (PreH9 : (i < nums_size_pre)) (PreH10 : (0 <= num)) (PreH11 : (num <= i)) (PreH12 : (current = (Znth (i) (input_l) (0)))) (PreH13 : (current > 10)) (PreH14 : (INT_MIN <= current)) (PreH15 : (current <= INT_MAX)) (PreH16 : (1 <= first)) (PreH17 : (first < 10)) (PreH18 : (last = (current % ( 10 ) ))) (PreH19 : (first_digit_state_146 current first )) (PreH20 : (special_filter_prefix_146 input_l i num )) ,
+  TT && emp 
+|--
+  “ (special_filter_prefix_146 input_l (i + 1 ) (num + 1 ) ) ”
+  &&  emp
+).
+
+Definition specialFilter_entail_wit_7_split_goal_1 := 
+forall (nums_size_pre: Z) (input_l: (@list Z)) (i: Z) (num: Z) (current: Z) (first: Z) (last: Z) (PreH1 : ((last % ( 2 ) ) = 1)) (PreH2 : ((first % ( 2 ) ) = 1)) (PreH3 : (0 <= nums_size_pre)) (PreH4 : (nums_size_pre < INT_MAX)) (PreH5 : (nums_size_pre = (Zlength (input_l)))) (PreH6 : (problem_146_pre_z input_l )) (PreH7 : (special_filter_safe_146 input_l )) (PreH8 : (0 <= i)) (PreH9 : (i < nums_size_pre)) (PreH10 : (0 <= num)) (PreH11 : (num <= i)) (PreH12 : (current = (Znth (i) (input_l) (0)))) (PreH13 : (current > 10)) (PreH14 : (INT_MIN <= current)) (PreH15 : (current <= INT_MAX)) (PreH16 : (1 <= first)) (PreH17 : (first < 10)) (PreH18 : (last = (current % ( 10 ) ))) (PreH19 : (first_digit_state_146 current first )) (PreH20 : (special_filter_prefix_146 input_l i num )) ,
+  TT && emp 
+|--
+  “ (special_filter_prefix_146 input_l (i + 1 ) (num + 1 ) ) ”
+.
+
+Definition specialFilter_entail_wit_8_1 := 
+forall (nums_size_pre: Z) (nums_pre: Z) (input_l: (@list Z)) (i: Z) (num: Z) (current: Z) (first: Z) (last: Z) (PreH1 : ((last % ( 2 ) ) <> 1)) (PreH2 : ((first % ( 2 ) ) = 1)) (PreH3 : (0 <= nums_size_pre)) (PreH4 : (nums_size_pre < INT_MAX)) (PreH5 : (nums_size_pre = (Zlength (input_l)))) (PreH6 : (problem_146_pre_z input_l )) (PreH7 : (special_filter_safe_146 input_l )) (PreH8 : (0 <= i)) (PreH9 : (i < nums_size_pre)) (PreH10 : (0 <= num)) (PreH11 : (num <= i)) (PreH12 : (current = (Znth (i) (input_l) (0)))) (PreH13 : (current > 10)) (PreH14 : (INT_MIN <= current)) (PreH15 : (current <= INT_MAX)) (PreH16 : (1 <= first)) (PreH17 : (first < 10)) (PreH18 : (last = (current % ( 10 ) ))) (PreH19 : (first_digit_state_146 current first )) (PreH20 : (special_filter_prefix_146 input_l i num )) ,
+  (IntArray.full nums_pre nums_size_pre input_l )
+|--
+  (“ (0 <= nums_size_pre) ” 
+  &&  “ (nums_size_pre < INT_MAX) ” 
+  &&  “ (nums_size_pre = (Zlength (input_l))) ” 
+  &&  “ (problem_146_pre_z input_l ) ” 
+  &&  “ (special_filter_safe_146 input_l ) ” 
+  &&  “ (0 <= i) ” 
+  &&  “ (i < nums_size_pre) ” 
+  &&  “ (0 <= num) ” 
+  &&  “ (num <= i) ” 
+  &&  “ (current = (Znth (i) (input_l) (0))) ” 
+  &&  “ (current > 10) ” 
+  &&  “ (first_digit_state_146 current first ) ” 
+  &&  “ (first < 10) ” 
+  &&  “ (last = (current % ( 10 ) )) ” 
+  &&  “ ((last % ( 2 ) ) <> 1) ” 
+  &&  “ (special_filter_prefix_146 input_l (i + 1 ) num ) ”
+  &&  (IntArray.full nums_pre nums_size_pre input_l ))
+  ||
+  (“ (0 <= nums_size_pre) ” 
+  &&  “ (nums_size_pre < INT_MAX) ” 
+  &&  “ (nums_size_pre = (Zlength (input_l))) ” 
+  &&  “ (problem_146_pre_z input_l ) ” 
+  &&  “ (special_filter_safe_146 input_l ) ” 
+  &&  “ (0 <= i) ” 
+  &&  “ (i < nums_size_pre) ” 
+  &&  “ (0 <= num) ” 
+  &&  “ (num <= i) ” 
+  &&  “ (current = (Znth (i) (input_l) (0))) ” 
+  &&  “ (current > 10) ” 
+  &&  “ (first_digit_state_146 current first ) ” 
+  &&  “ (first < 10) ” 
+  &&  “ (last = (current % ( 10 ) )) ” 
+  &&  “ ((first % ( 2 ) ) <> 1) ” 
+  &&  “ (special_filter_prefix_146 input_l (i + 1 ) num ) ”
+  &&  (IntArray.full nums_pre nums_size_pre input_l ))
+.
+
+Definition specialFilter_entail_wit_8_2 := 
+forall (nums_size_pre: Z) (nums_pre: Z) (input_l: (@list Z)) (i: Z) (num: Z) (current: Z) (first: Z) (last: Z) (PreH1 : ((first % ( 2 ) ) <> 1)) (PreH2 : (0 <= nums_size_pre)) (PreH3 : (nums_size_pre < INT_MAX)) (PreH4 : (nums_size_pre = (Zlength (input_l)))) (PreH5 : (problem_146_pre_z input_l )) (PreH6 : (special_filter_safe_146 input_l )) (PreH7 : (0 <= i)) (PreH8 : (i < nums_size_pre)) (PreH9 : (0 <= num)) (PreH10 : (num <= i)) (PreH11 : (current = (Znth (i) (input_l) (0)))) (PreH12 : (current > 10)) (PreH13 : (INT_MIN <= current)) (PreH14 : (current <= INT_MAX)) (PreH15 : (1 <= first)) (PreH16 : (first < 10)) (PreH17 : (last = (current % ( 10 ) ))) (PreH18 : (first_digit_state_146 current first )) (PreH19 : (special_filter_prefix_146 input_l i num )) ,
+  (IntArray.full nums_pre nums_size_pre input_l )
+|--
+  (“ (0 <= nums_size_pre) ” 
+  &&  “ (nums_size_pre < INT_MAX) ” 
+  &&  “ (nums_size_pre = (Zlength (input_l))) ” 
+  &&  “ (problem_146_pre_z input_l ) ” 
+  &&  “ (special_filter_safe_146 input_l ) ” 
+  &&  “ (0 <= i) ” 
+  &&  “ (i < nums_size_pre) ” 
+  &&  “ (0 <= num) ” 
+  &&  “ (num <= i) ” 
+  &&  “ (current = (Znth (i) (input_l) (0))) ” 
+  &&  “ (current > 10) ” 
+  &&  “ (first_digit_state_146 current first ) ” 
+  &&  “ (first < 10) ” 
+  &&  “ (last = (current % ( 10 ) )) ” 
+  &&  “ ((last % ( 2 ) ) <> 1) ” 
+  &&  “ (special_filter_prefix_146 input_l (i + 1 ) num ) ”
+  &&  (IntArray.full nums_pre nums_size_pre input_l ))
+  ||
+  (“ (0 <= nums_size_pre) ” 
+  &&  “ (nums_size_pre < INT_MAX) ” 
+  &&  “ (nums_size_pre = (Zlength (input_l))) ” 
+  &&  “ (problem_146_pre_z input_l ) ” 
+  &&  “ (special_filter_safe_146 input_l ) ” 
+  &&  “ (0 <= i) ” 
+  &&  “ (i < nums_size_pre) ” 
+  &&  “ (0 <= num) ” 
+  &&  “ (num <= i) ” 
+  &&  “ (current = (Znth (i) (input_l) (0))) ” 
+  &&  “ (current > 10) ” 
+  &&  “ (first_digit_state_146 current first ) ” 
+  &&  “ (first < 10) ” 
+  &&  “ (last = (current % ( 10 ) )) ” 
+  &&  “ ((first % ( 2 ) ) <> 1) ” 
+  &&  “ (special_filter_prefix_146 input_l (i + 1 ) num ) ”
+  &&  (IntArray.full nums_pre nums_size_pre input_l ))
+.
+
+Definition specialFilter_entail_wit_9 := 
+(
+forall (nums_size_pre: Z) (nums_pre: Z) (input_l: (@list Z)) (i: Z) (num: Z) (current: Z) (PreH1 : (current <= 10)) (PreH2 : (0 <= nums_size_pre)) (PreH3 : (nums_size_pre < INT_MAX)) (PreH4 : (nums_size_pre = (Zlength (input_l)))) (PreH5 : (problem_146_pre_z input_l )) (PreH6 : (special_filter_safe_146 input_l )) (PreH7 : (0 <= i)) (PreH8 : (i < nums_size_pre)) (PreH9 : (0 <= num)) (PreH10 : (num <= i)) (PreH11 : (current = (Znth (i) (input_l) (0)))) (PreH12 : (INT_MIN <= current)) (PreH13 : (current <= INT_MAX)) (PreH14 : (special_filter_prefix_146 input_l i num )) ,
+  (IntArray.full nums_pre nums_size_pre input_l )
+|--
+  “ (0 <= nums_size_pre) ” 
+  &&  “ (nums_size_pre < INT_MAX) ” 
+  &&  “ (nums_size_pre = (Zlength (input_l))) ” 
+  &&  “ (problem_146_pre_z input_l ) ” 
+  &&  “ (special_filter_safe_146 input_l ) ” 
+  &&  “ (0 <= i) ” 
+  &&  “ (i < nums_size_pre) ” 
+  &&  “ (0 <= num) ” 
+  &&  “ (num <= i) ” 
+  &&  “ (current = (Znth (i) (input_l) (0))) ” 
+  &&  “ (current <= 10) ” 
+  &&  “ (special_filter_prefix_146 input_l (i + 1 ) num ) ”
+  &&  (IntArray.full nums_pre nums_size_pre input_l )
+) \/
+(
+forall (nums_size_pre: Z) (input_l: (@list Z)) (i: Z) (num: Z) (current: Z) (PreH1 : (current <= 10)) (PreH2 : (0 <= nums_size_pre)) (PreH3 : (nums_size_pre < INT_MAX)) (PreH4 : (nums_size_pre = (Zlength (input_l)))) (PreH5 : (problem_146_pre_z input_l )) (PreH6 : (special_filter_safe_146 input_l )) (PreH7 : (0 <= i)) (PreH8 : (i < nums_size_pre)) (PreH9 : (0 <= num)) (PreH10 : (num <= i)) (PreH11 : (current = (Znth (i) (input_l) (0)))) (PreH12 : (INT_MIN <= current)) (PreH13 : (current <= INT_MAX)) (PreH14 : (special_filter_prefix_146 input_l i num )) ,
+  TT && emp 
+|--
+  “ (special_filter_prefix_146 input_l (i + 1 ) num ) ”
+  &&  emp
+).
+
+Definition specialFilter_entail_wit_9_split_goal_1 := 
+forall (nums_size_pre: Z) (input_l: (@list Z)) (i: Z) (num: Z) (current: Z) (PreH1 : (current <= 10)) (PreH2 : (0 <= nums_size_pre)) (PreH3 : (nums_size_pre < INT_MAX)) (PreH4 : (nums_size_pre = (Zlength (input_l)))) (PreH5 : (problem_146_pre_z input_l )) (PreH6 : (special_filter_safe_146 input_l )) (PreH7 : (0 <= i)) (PreH8 : (i < nums_size_pre)) (PreH9 : (0 <= num)) (PreH10 : (num <= i)) (PreH11 : (current = (Znth (i) (input_l) (0)))) (PreH12 : (INT_MIN <= current)) (PreH13 : (current <= INT_MAX)) (PreH14 : (special_filter_prefix_146 input_l i num )) ,
+  TT && emp 
+|--
+  “ (special_filter_prefix_146 input_l (i + 1 ) num ) ”
+.
+
+Definition specialFilter_entail_wit_10_1 := 
+forall (nums_size_pre: Z) (nums_pre: Z) (input_l: (@list Z)) (i: Z) (num: Z) (current: Z) (first: Z) (last: Z) (PreH1 : (0 <= nums_size_pre)) (PreH2 : (nums_size_pre < INT_MAX)) (PreH3 : (nums_size_pre = (Zlength (input_l)))) (PreH4 : (problem_146_pre_z input_l )) (PreH5 : (special_filter_safe_146 input_l )) (PreH6 : (0 <= i)) (PreH7 : (i < nums_size_pre)) (PreH8 : (0 <= num)) (PreH9 : (num <= (i + 1 ))) (PreH10 : (current = (Znth (i) (input_l) (0)))) (PreH11 : (current > 10)) (PreH12 : (first_digit_state_146 current first )) (PreH13 : (first < 10)) (PreH14 : (last = (current % ( 10 ) ))) (PreH15 : ((first % ( 2 ) ) = 1)) (PreH16 : ((last % ( 2 ) ) = 1)) (PreH17 : (special_filter_prefix_146 input_l (i + 1 ) num )) ,
+  (IntArray.full nums_pre nums_size_pre input_l )
+|--
+  “ (0 <= nums_size_pre) ” 
+  &&  “ (nums_size_pre < INT_MAX) ” 
+  &&  “ (nums_size_pre = (Zlength (input_l))) ” 
+  &&  “ (problem_146_pre_z input_l ) ” 
+  &&  “ (special_filter_safe_146 input_l ) ” 
+  &&  “ (0 <= (i + 1 )) ” 
+  &&  “ ((i + 1 ) <= nums_size_pre) ” 
+  &&  “ (0 <= num) ” 
+  &&  “ (num <= (i + 1 )) ” 
+  &&  “ (special_filter_prefix_146 input_l (i + 1 ) num ) ”
+  &&  (IntArray.full nums_pre nums_size_pre input_l )
+.
+
+Definition specialFilter_entail_wit_10_2 := 
+forall (nums_size_pre: Z) (nums_pre: Z) (input_l: (@list Z)) (i: Z) (num: Z) (current: Z) (first: Z) (last: Z) (PreH1 : (0 <= nums_size_pre)) (PreH2 : (nums_size_pre < INT_MAX)) (PreH3 : (nums_size_pre = (Zlength (input_l)))) (PreH4 : (problem_146_pre_z input_l )) (PreH5 : (special_filter_safe_146 input_l )) (PreH6 : (0 <= i)) (PreH7 : (i < nums_size_pre)) (PreH8 : (0 <= num)) (PreH9 : (num <= i)) (PreH10 : (current = (Znth (i) (input_l) (0)))) (PreH11 : (current > 10)) (PreH12 : (first_digit_state_146 current first )) (PreH13 : (first < 10)) (PreH14 : (last = (current % ( 10 ) ))) (PreH15 : ((last % ( 2 ) ) <> 1)) (PreH16 : (special_filter_prefix_146 input_l (i + 1 ) num )) ,
+  (IntArray.full nums_pre nums_size_pre input_l )
+|--
+  “ (0 <= nums_size_pre) ” 
+  &&  “ (nums_size_pre < INT_MAX) ” 
+  &&  “ (nums_size_pre = (Zlength (input_l))) ” 
+  &&  “ (problem_146_pre_z input_l ) ” 
+  &&  “ (special_filter_safe_146 input_l ) ” 
+  &&  “ (0 <= (i + 1 )) ” 
+  &&  “ ((i + 1 ) <= nums_size_pre) ” 
+  &&  “ (0 <= num) ” 
+  &&  “ (num <= (i + 1 )) ” 
+  &&  “ (special_filter_prefix_146 input_l (i + 1 ) num ) ”
+  &&  (IntArray.full nums_pre nums_size_pre input_l )
+.
+
+Definition specialFilter_entail_wit_10_3 := 
+forall (nums_size_pre: Z) (nums_pre: Z) (input_l: (@list Z)) (i: Z) (num: Z) (current: Z) (first: Z) (last: Z) (PreH1 : (0 <= nums_size_pre)) (PreH2 : (nums_size_pre < INT_MAX)) (PreH3 : (nums_size_pre = (Zlength (input_l)))) (PreH4 : (problem_146_pre_z input_l )) (PreH5 : (special_filter_safe_146 input_l )) (PreH6 : (0 <= i)) (PreH7 : (i < nums_size_pre)) (PreH8 : (0 <= num)) (PreH9 : (num <= i)) (PreH10 : (current = (Znth (i) (input_l) (0)))) (PreH11 : (current > 10)) (PreH12 : (first_digit_state_146 current first )) (PreH13 : (first < 10)) (PreH14 : (last = (current % ( 10 ) ))) (PreH15 : ((first % ( 2 ) ) <> 1)) (PreH16 : (special_filter_prefix_146 input_l (i + 1 ) num )) ,
+  (IntArray.full nums_pre nums_size_pre input_l )
+|--
+  “ (0 <= nums_size_pre) ” 
+  &&  “ (nums_size_pre < INT_MAX) ” 
+  &&  “ (nums_size_pre = (Zlength (input_l))) ” 
+  &&  “ (problem_146_pre_z input_l ) ” 
+  &&  “ (special_filter_safe_146 input_l ) ” 
+  &&  “ (0 <= (i + 1 )) ” 
+  &&  “ ((i + 1 ) <= nums_size_pre) ” 
+  &&  “ (0 <= num) ” 
+  &&  “ (num <= (i + 1 )) ” 
+  &&  “ (special_filter_prefix_146 input_l (i + 1 ) num ) ”
+  &&  (IntArray.full nums_pre nums_size_pre input_l )
+.
+
+Definition specialFilter_entail_wit_10_4 := 
+forall (nums_size_pre: Z) (nums_pre: Z) (input_l: (@list Z)) (i: Z) (num: Z) (current: Z) (PreH1 : (0 <= nums_size_pre)) (PreH2 : (nums_size_pre < INT_MAX)) (PreH3 : (nums_size_pre = (Zlength (input_l)))) (PreH4 : (problem_146_pre_z input_l )) (PreH5 : (special_filter_safe_146 input_l )) (PreH6 : (0 <= i)) (PreH7 : (i < nums_size_pre)) (PreH8 : (0 <= num)) (PreH9 : (num <= i)) (PreH10 : (current = (Znth (i) (input_l) (0)))) (PreH11 : (current <= 10)) (PreH12 : (special_filter_prefix_146 input_l (i + 1 ) num )) ,
+  (IntArray.full nums_pre nums_size_pre input_l )
+|--
+  “ (0 <= nums_size_pre) ” 
+  &&  “ (nums_size_pre < INT_MAX) ” 
+  &&  “ (nums_size_pre = (Zlength (input_l))) ” 
+  &&  “ (problem_146_pre_z input_l ) ” 
+  &&  “ (special_filter_safe_146 input_l ) ” 
+  &&  “ (0 <= (i + 1 )) ” 
+  &&  “ ((i + 1 ) <= nums_size_pre) ” 
+  &&  “ (0 <= num) ” 
+  &&  “ (num <= (i + 1 )) ” 
+  &&  “ (special_filter_prefix_146 input_l (i + 1 ) num ) ”
+  &&  (IntArray.full nums_pre nums_size_pre input_l )
+.
+
+Definition specialFilter_return_wit_1 := 
+(
+forall (nums_size_pre: Z) (nums_pre: Z) (input_l: (@list Z)) (num: Z) (i: Z) (PreH1 : (i >= nums_size_pre)) (PreH2 : (0 <= nums_size_pre)) (PreH3 : (nums_size_pre < INT_MAX)) (PreH4 : (nums_size_pre = (Zlength (input_l)))) (PreH5 : (problem_146_pre_z input_l )) (PreH6 : (special_filter_safe_146 input_l )) (PreH7 : (0 <= i)) (PreH8 : (i <= nums_size_pre)) (PreH9 : (0 <= num)) (PreH10 : (num <= i)) (PreH11 : (special_filter_prefix_146 input_l i num )) ,
+  (IntArray.full nums_pre nums_size_pre input_l )
+|--
+  “ (problem_146_spec_z input_l num ) ”
+  &&  (IntArray.full nums_pre nums_size_pre input_l )
+) \/
+(
+forall (nums_size_pre: Z) (input_l: (@list Z)) (num: Z) (i: Z) (PreH1 : (i >= nums_size_pre)) (PreH2 : (0 <= nums_size_pre)) (PreH3 : (nums_size_pre < INT_MAX)) (PreH4 : (nums_size_pre = (Zlength (input_l)))) (PreH5 : (problem_146_pre_z input_l )) (PreH6 : (special_filter_safe_146 input_l )) (PreH7 : (0 <= i)) (PreH8 : (i <= nums_size_pre)) (PreH9 : (0 <= num)) (PreH10 : (num <= i)) (PreH11 : (special_filter_prefix_146 input_l i num )) ,
+  TT && emp 
+|--
+  “ (problem_146_spec_z input_l num ) ”
+  &&  emp
+).
+
+Definition specialFilter_return_wit_1_split_goal_1 := 
+forall (nums_size_pre: Z) (input_l: (@list Z)) (num: Z) (i: Z) (PreH1 : (i >= nums_size_pre)) (PreH2 : (0 <= nums_size_pre)) (PreH3 : (nums_size_pre < INT_MAX)) (PreH4 : (nums_size_pre = (Zlength (input_l)))) (PreH5 : (problem_146_pre_z input_l )) (PreH6 : (special_filter_safe_146 input_l )) (PreH7 : (0 <= i)) (PreH8 : (i <= nums_size_pre)) (PreH9 : (0 <= num)) (PreH10 : (num <= i)) (PreH11 : (special_filter_prefix_146 input_l i num )) ,
+  TT && emp 
+|--
+  “ (problem_146_spec_z input_l num ) ”
+.
+
+Definition specialFilter_partial_solve_wit_1 := 
+forall (nums_size_pre: Z) (nums_pre: Z) (input_l: (@list Z)) (num: Z) (i: Z) (PreH1 : (i < nums_size_pre)) (PreH2 : (0 <= nums_size_pre)) (PreH3 : (nums_size_pre < INT_MAX)) (PreH4 : (nums_size_pre = (Zlength (input_l)))) (PreH5 : (problem_146_pre_z input_l )) (PreH6 : (special_filter_safe_146 input_l )) (PreH7 : (0 <= i)) (PreH8 : (i <= nums_size_pre)) (PreH9 : (0 <= num)) (PreH10 : (num <= i)) (PreH11 : (special_filter_prefix_146 input_l i num )) ,
+  (IntArray.full nums_pre nums_size_pre input_l )
+|--
+  “ (i < nums_size_pre) ” 
+  &&  “ (0 <= nums_size_pre) ” 
+  &&  “ (nums_size_pre < INT_MAX) ” 
+  &&  “ (nums_size_pre = (Zlength (input_l))) ” 
+  &&  “ (problem_146_pre_z input_l ) ” 
+  &&  “ (special_filter_safe_146 input_l ) ” 
+  &&  “ (0 <= i) ” 
+  &&  “ (i <= nums_size_pre) ” 
+  &&  “ (0 <= num) ” 
+  &&  “ (num <= i) ” 
+  &&  “ (special_filter_prefix_146 input_l i num ) ”
+  &&  (((nums_pre + (i * sizeof(INT) ) )) # Int  |-> (Znth i input_l 0))
+  **  (IntArray.missing_i nums_pre i 0 nums_size_pre input_l )
+.
+
+Module Type VC_Correct.
+
+Include int_array_Strategy_Correct.
+Include uint_array_Strategy_Correct.
+Include undef_uint_array_Strategy_Correct.
+Include array_shape_Strategy_Correct.
+
+Axiom proof_of_specialFilter_safety_wit_1 : specialFilter_safety_wit_1.
+Axiom proof_of_specialFilter_safety_wit_2 : specialFilter_safety_wit_2.
+Axiom proof_of_specialFilter_safety_wit_3 : specialFilter_safety_wit_3.
+Axiom proof_of_specialFilter_safety_wit_4 : specialFilter_safety_wit_4.
+Axiom proof_of_specialFilter_safety_wit_5 : specialFilter_safety_wit_5.
+Axiom proof_of_specialFilter_safety_wit_6 : specialFilter_safety_wit_6.
+Axiom proof_of_specialFilter_safety_wit_7 : specialFilter_safety_wit_7.
+Axiom proof_of_specialFilter_safety_wit_8 : specialFilter_safety_wit_8.
+Axiom proof_of_specialFilter_safety_wit_9 : specialFilter_safety_wit_9.
+Axiom proof_of_specialFilter_safety_wit_10 : specialFilter_safety_wit_10.
+Axiom proof_of_specialFilter_safety_wit_11 : specialFilter_safety_wit_11.
+Axiom proof_of_specialFilter_safety_wit_12 : specialFilter_safety_wit_12.
+Axiom proof_of_specialFilter_safety_wit_13 : specialFilter_safety_wit_13.
+Axiom proof_of_specialFilter_safety_wit_14 : specialFilter_safety_wit_14.
+Axiom proof_of_specialFilter_safety_wit_15 : specialFilter_safety_wit_15.
+Axiom proof_of_specialFilter_safety_wit_16 : specialFilter_safety_wit_16.
+Axiom proof_of_specialFilter_safety_wit_17 : specialFilter_safety_wit_17.
+Axiom proof_of_specialFilter_safety_wit_18 : specialFilter_safety_wit_18.
+Axiom proof_of_specialFilter_safety_wit_19 : specialFilter_safety_wit_19.
+Axiom proof_of_specialFilter_safety_wit_20 : specialFilter_safety_wit_20.
+Axiom proof_of_specialFilter_entail_wit_1 : specialFilter_entail_wit_1.
+Axiom proof_of_specialFilter_entail_wit_2 : specialFilter_entail_wit_2.
+Axiom proof_of_specialFilter_entail_wit_3 : specialFilter_entail_wit_3.
+Axiom proof_of_specialFilter_entail_wit_4 : specialFilter_entail_wit_4.
+Axiom proof_of_specialFilter_entail_wit_5 : specialFilter_entail_wit_5.
+Axiom proof_of_specialFilter_entail_wit_6 : specialFilter_entail_wit_6.
+Axiom proof_of_specialFilter_entail_wit_7 : specialFilter_entail_wit_7.
+Axiom proof_of_specialFilter_entail_wit_8_1 : specialFilter_entail_wit_8_1.
+Axiom proof_of_specialFilter_entail_wit_8_2 : specialFilter_entail_wit_8_2.
+Axiom proof_of_specialFilter_entail_wit_9 : specialFilter_entail_wit_9.
+Axiom proof_of_specialFilter_entail_wit_10_1 : specialFilter_entail_wit_10_1.
+Axiom proof_of_specialFilter_entail_wit_10_2 : specialFilter_entail_wit_10_2.
+Axiom proof_of_specialFilter_entail_wit_10_3 : specialFilter_entail_wit_10_3.
+Axiom proof_of_specialFilter_entail_wit_10_4 : specialFilter_entail_wit_10_4.
+Axiom proof_of_specialFilter_return_wit_1 : specialFilter_return_wit_1.
+Axiom proof_of_specialFilter_partial_solve_wit_1 : specialFilter_partial_solve_wit_1.
+
+End VC_Correct.
