QCP_examples/humaneval/spec_logic_rewrite_c_files/C_146_proof_manual.v
@@ -1,0 +1,190 @@
+Require Import Coq.ZArith.ZArith.
+Require Import Coq.Bool.Bool.
+Require Import Coq.Strings.String.
+Require Import Coq.Strings.Ascii.
+Require Import Coq.Lists.List.
+Require Import Coq.Classes.RelationClasses.
+Require Import Coq.Classes.Morphisms.
+Require Import Coq.micromega.Psatz.
+Require Import Coq.Sorting.Permutation.
+From AUXLib Require Import int_auto Axioms Feq Idents ListLib VMap.
+Require Import SetsClass.SetsClass. Import SetsNotation.
+From SimpleC.SL Require Import Mem SeparationLogic.
+From SimpleC.EE Require Import C_146_goal.
+From SimpleC.EE Require Import C_146_proof_auto.
+Require Import Logic.LogicGenerator.demo932.Interface.
+Local Open Scope Z_scope.
+Local Open Scope sets.
+Local Open Scope string_scope.
+Local Open Scope list.
+Import naive_C_Rules.
+Require Import coins_146.
+Local Open Scope sac.
+
+Lemma proof_of_specialFilter_entail_wit_1_split_goal_1 : specialFilter_entail_wit_1_split_goal_1.
+Proof.
+  unfold specialFilter_entail_wit_1_split_goal_1; intros.
+  pre_process; entailer!.
+  apply special_filter_prefix_init_146.
+Qed.
+
+Lemma proof_of_specialFilter_entail_wit_1 : specialFilter_entail_wit_1.
+Proof.
+  unfold specialFilter_entail_wit_1; right; intros.
+  pre_process; entailer!.
+  apply special_filter_prefix_init_146.
+Qed.
+
+Lemma proof_of_specialFilter_entail_wit_2_split_goal_1 : specialFilter_entail_wit_2_split_goal_1.
+Proof.
+  unfold specialFilter_entail_wit_2_split_goal_1; intros.
+  pre_process; entailer!.
+  pose proof (special_filter_safe_Znth_range_146 input_l i PreH6 ltac:(lia)).
+  lia.
+Qed.
+
+Lemma proof_of_specialFilter_entail_wit_2_split_goal_2 : specialFilter_entail_wit_2_split_goal_2.
+Proof.
+  unfold specialFilter_entail_wit_2_split_goal_2; intros.
+  pre_process; entailer!.
+  pose proof (special_filter_safe_Znth_range_146 input_l i PreH6 ltac:(lia)).
+  lia.
+Qed.
+
+Lemma proof_of_specialFilter_entail_wit_2_split_goal_3 : specialFilter_entail_wit_2_split_goal_3.
+Proof.
+  unfold specialFilter_entail_wit_2_split_goal_3; intros.
+  pre_process; entailer!.
+Qed.
+
+Lemma proof_of_specialFilter_entail_wit_2 : specialFilter_entail_wit_2.
+Proof.
+  unfold specialFilter_entail_wit_2; right; intros.
+  pre_process; entailer!;
+    try pose proof (special_filter_safe_Znth_range_146 input_l i PreH6 ltac:(lia));
+    lia.
+Qed.
+
+Lemma proof_of_specialFilter_entail_wit_3_split_goal_1 : specialFilter_entail_wit_3_split_goal_1.
+Proof.
+  unfold specialFilter_entail_wit_3_split_goal_1; intros.
+  pre_process; entailer!.
+  subst current.
+  eapply special_filter_safe_Znth_first_init_146; eauto; lia.
+Qed.
+
+Lemma proof_of_specialFilter_entail_wit_3 : specialFilter_entail_wit_3.
+Proof.
+  unfold specialFilter_entail_wit_3; right; intros.
+  pre_process; entailer!.
+  subst current.
+  eapply special_filter_safe_Znth_first_init_146; eauto; lia.
+Qed.
+
+Lemma proof_of_specialFilter_entail_wit_5_split_goal_1 : specialFilter_entail_wit_5_split_goal_1.
+Proof.
+  unfold specialFilter_entail_wit_5_split_goal_1; intros.
+  pre_process; entailer!.
+  pose proof (first_digit_state_step_146 current first PreH18 ltac:(lia)) as Hnext.
+  exact Hnext.
+Qed.
+
+Lemma proof_of_specialFilter_entail_wit_5_split_goal_2 : specialFilter_entail_wit_5_split_goal_2.
+Proof.
+  unfold specialFilter_entail_wit_5_split_goal_2; intros.
+  pre_process; entailer!.
+  pose proof (first_digit_state_step_146 current first PreH18 ltac:(lia)) as Hnext.
+  unfold first_digit_state_146 in Hnext.
+  lia.
+Qed.
+
+Lemma proof_of_specialFilter_entail_wit_5_split_goal_3 : specialFilter_entail_wit_5_split_goal_3.
+Proof.
+  unfold specialFilter_entail_wit_5_split_goal_3; intros.
+  pre_process; entailer!.
+  pose proof (first_digit_state_step_146 current first PreH18 ltac:(lia)) as Hnext.
+  unfold first_digit_state_146 in Hnext.
+  lia.
+Qed.
+
+Lemma proof_of_specialFilter_entail_wit_5 : specialFilter_entail_wit_5.
+Proof.
+  unfold specialFilter_entail_wit_5; right; intros.
+  pre_process; entailer!;
+    pose proof (first_digit_state_step_146 current first PreH18 ltac:(lia)) as Hnext;
+    try exact Hnext; unfold first_digit_state_146 in Hnext; lia.
+Qed.
+
+Lemma proof_of_specialFilter_entail_wit_7_split_goal_1 : specialFilter_entail_wit_7_split_goal_1.
+Proof.
+  unfold specialFilter_entail_wit_7_split_goal_1; intros.
+  pre_process; entailer!.
+  eapply special_filter_prefix_step_one_146; [lia | exact PreH20 |].
+  replace (Znth i input_l 0) with current by lia.
+  eapply (special_score_one_from_scan_146 input_l i current first last); eauto; lia.
+Qed.
+
+Lemma proof_of_specialFilter_entail_wit_7 : specialFilter_entail_wit_7.
+Proof.
+  unfold specialFilter_entail_wit_7; right; intros.
+  pre_process; entailer!.
+  eapply special_filter_prefix_step_one_146; [lia | exact PreH20 |].
+  replace (Znth i input_l 0) with current by lia.
+  eapply (special_score_one_from_scan_146 input_l i current first last); eauto; lia.
+Qed.
+
+Lemma proof_of_specialFilter_entail_wit_8_1 : specialFilter_entail_wit_8_1.
+Proof.
+  unfold specialFilter_entail_wit_8_1; intros.
+  rewrite <- derivable1_orp_intros1.
+  pre_process; entailer!.
+  eapply special_filter_prefix_step_zero_146; [lia | exact PreH20 |].
+  replace (Znth i input_l 0) with current by lia.
+  eapply (special_score_zero_from_scan_last_146 input_l i current first last); eauto; lia.
+Qed.
+
+Lemma proof_of_specialFilter_entail_wit_8_2 : specialFilter_entail_wit_8_2.
+Proof.
+  unfold specialFilter_entail_wit_8_2; intros.
+  rewrite <- derivable1_orp_intros2.
+  pre_process; entailer!.
+  eapply special_filter_prefix_step_zero_146; [lia | exact PreH19 |].
+  replace (Znth i input_l 0) with current by lia.
+  eapply (special_score_zero_from_scan_first_146 input_l i current first last); eauto; lia.
+Qed.
+
+Lemma proof_of_specialFilter_entail_wit_9_split_goal_1 : specialFilter_entail_wit_9_split_goal_1.
+Proof.
+  unfold specialFilter_entail_wit_9_split_goal_1; intros.
+  pre_process; entailer!.
+  eapply special_filter_prefix_step_zero_146; [lia | exact PreH14 |].
+  subst current.
+  eapply special_filter_safe_Znth_small_score_146; eauto; lia.
+Qed.
+
+Lemma proof_of_specialFilter_entail_wit_9 : specialFilter_entail_wit_9.
+Proof.
+  unfold specialFilter_entail_wit_9; right; intros.
+  pre_process; entailer!.
+  eapply special_filter_prefix_step_zero_146; [lia | exact PreH14 |].
+  subst current.
+  eapply special_filter_safe_Znth_small_score_146; eauto; lia.
+Qed.
+
+Lemma proof_of_specialFilter_return_wit_1_split_goal_1 : specialFilter_return_wit_1_split_goal_1.
+Proof.
+  unfold specialFilter_return_wit_1_split_goal_1; intros.
+  pre_process; entailer!.
+  apply special_filter_prefix_final_146.
+  replace (Zlength input_l) with i by lia.
+  exact PreH11.
+Qed.
+
+Lemma proof_of_specialFilter_return_wit_1 : specialFilter_return_wit_1.
+Proof.
+  unfold specialFilter_return_wit_1; right; intros.
+  pre_process; entailer!.
+  apply special_filter_prefix_final_146.
+  replace (Zlength input_l) with i by lia.
+  exact PreH11.
+Qed.
