QCP_examples/humaneval/spec_logic_rewrite_c_files/coins_146.v
@@ -1,0 +1,365 @@
+Load "../spec/146".
+
+Require Import Coq.Lists.List.
+Require Import Coq.ZArith.ZArith.
+Require Import Coq.ZArith.Zquot.
+Require Import Coq.micromega.Lia.
+From AUXLib Require Import ListLib.
+From SimpleC.SL Require Import IntLib.
+
+Import ListNotations.
+Local Open Scope Z_scope.
+
+Definition problem_146_pre_z (nums : list Z) : Prop :=
+  problem_146_pre nums.
+
+Definition problem_146_spec_z (nums : list Z) (out : Z) : Prop :=
+  problem_146_spec nums out.
+
+Definition first_digit_state_146 (x first : Z) : Prop :=
+  0 <= first <= x /\
+  0 < x /\
+  1 <= first /\
+  exists k tail,
+    0 <= k /\
+    0 <= tail < 10 ^ k /\
+    x = first * 10 ^ k + tail.
+
+Definition special_filter_safe_146 (nums : list Z) : Prop :=
+  Forall
+    (fun x =>
+      INT_MIN <= x <= INT_MAX /\
+      (x <= 10 -> special_number_score x 0) /\
+      (10 < x -> first_digit_state_146 x x) /\
+      (forall first last_digit score,
+        first_digit_state_146 x first ->
+        first < 10 ->
+        last_digit = Z.rem x 10 ->
+        ((10 < x /\
+          Z.odd first = true /\
+          Z.odd last_digit = true /\
+          score = 1) \/
+         ((x <= 10 \/
+           Z.odd first = false \/
+           Z.odd last_digit = false) /\
+          score = 0)) ->
+        special_number_score x score))
+    nums.
+
+Definition special_filter_prefix_146 (nums : list Z) (i count : Z) : Prop :=
+  exists scores,
+    0 <= i <= Zlength nums /\
+    Forall2 special_number_score (sublist 0 i nums) scores /\
+    count = fold_left Z.add scores 0.
+
+Lemma special_filter_safe_Znth_range_146 : forall nums i,
+  special_filter_safe_146 nums ->
+  0 <= i < Zlength nums ->
+  INT_MIN <= Znth i nums 0 <= INT_MAX.
+Proof.
+  intros nums i Hsafe Hi.
+  unfold special_filter_safe_146 in Hsafe.
+  rewrite Forall_forall in Hsafe.
+  specialize (Hsafe (Znth i nums 0)).
+  assert (In (Znth i nums 0) nums).
+  { unfold Znth.
+    apply nth_In.
+    rewrite Zlength_correct in Hi.
+    lia. }
+  specialize (Hsafe H).
+  tauto.
+Qed.
+
+Lemma special_filter_safe_Znth_small_score_146 : forall nums i,
+  special_filter_safe_146 nums ->
+  0 <= i < Zlength nums ->
+  Znth i nums 0 <= 10 ->
+  special_number_score (Znth i nums 0) 0.
+Proof.
+  intros nums i Hsafe Hi Hsmall.
+  unfold special_filter_safe_146 in Hsafe.
+  rewrite Forall_forall in Hsafe.
+  specialize (Hsafe (Znth i nums 0)).
+  assert (In (Znth i nums 0) nums).
+  { unfold Znth.
+    apply nth_In.
+    rewrite Zlength_correct in Hi.
+    lia. }
+  specialize (Hsafe H) as [_ [Hscore _]].
+  apply Hscore; lia.
+Qed.
+
+Lemma special_filter_safe_Znth_first_init_146 : forall nums i,
+  special_filter_safe_146 nums ->
+  0 <= i < Zlength nums ->
+  10 < Znth i nums 0 ->
+  first_digit_state_146 (Znth i nums 0) (Znth i nums 0).
+Proof.
+  intros nums i Hsafe Hi Hgt.
+  unfold special_filter_safe_146 in Hsafe.
+  rewrite Forall_forall in Hsafe.
+  specialize (Hsafe (Znth i nums 0)).
+  assert (In (Znth i nums 0) nums).
+  { unfold Znth.
+    apply nth_In.
+    rewrite Zlength_correct in Hi.
+    lia. }
+  specialize (Hsafe H) as [_ [_ [Hinit _]]].
+  apply Hinit; lia.
+Qed.
+
+Lemma special_filter_safe_Znth_scan_score_146 : forall nums i first last_digit score,
+  special_filter_safe_146 nums ->
+  0 <= i < Zlength nums ->
+  first_digit_state_146 (Znth i nums 0) first ->
+  first < 10 ->
+  last_digit = Z.rem (Znth i nums 0) 10 ->
+  ((10 < Znth i nums 0 /\
+    Z.odd first = true /\
+    Z.odd last_digit = true /\
+    score = 1) \/
+   ((Znth i nums 0 <= 10 \/
+     Z.odd first = false \/
+     Z.odd last_digit = false) /\
+    score = 0)) ->
+  special_number_score (Znth i nums 0) score.
+Proof.
+  intros nums i first last_digit score Hsafe Hi Hstate Hfirst Hlast Hcase.
+  unfold special_filter_safe_146 in Hsafe.
+  rewrite Forall_forall in Hsafe.
+  specialize (Hsafe (Znth i nums 0)).
+  assert (In (Znth i nums 0) nums).
+  { unfold Znth.
+    apply nth_In.
+    rewrite Zlength_correct in Hi.
+    lia. }
+  specialize (Hsafe H) as [_ [_ [_ Hscore]]].
+  eapply Hscore; eauto.
+Qed.
+
+Lemma first_digit_state_step_146 : forall x first,
+  first_digit_state_146 x first ->
+  10 <= first ->
+  first_digit_state_146 x (Z.quot first 10).
+Proof.
+  intros x first Hstate Hfirst.
+  unfold first_digit_state_146 in *.
+  destruct Hstate as [Hbounds [Hxpos [Hfirst_pos [k [tail [Hk [Htail Hx]]]]]]].
+  repeat split.
+  - rewrite Z.quot_div_nonneg by lia.
+    apply Z.div_pos; lia.
+  - rewrite Z.quot_div_nonneg by lia.
+    apply Z.div_le_upper_bound; lia.
+  - lia.
+  - rewrite Z.quot_div_nonneg by lia.
+    apply Z.div_le_lower_bound; lia.
+  - exists (k + 1), (Z.rem first 10 * 10 ^ k + tail).
+    assert (Hrem_bounds : 0 <= Z.rem first 10 < 10).
+    { rewrite Z.rem_mod_nonneg by lia.
+      apply Z.mod_pos_bound; lia. }
+    assert (Hpow_pos : 0 < 10 ^ k).
+    { apply Z.pow_pos_nonneg; lia. }
+    repeat split.
+    + lia.
+    + nia.
+    + replace (10 ^ (k + 1)) with (10 * 10 ^ k)
+        by (replace (k + 1) with (Z.succ k) by lia;
+            rewrite Z.pow_succ_r by lia; ring).
+      nia.
+    + replace (10 ^ (k + 1)) with (10 * 10 ^ k)
+        by (replace (k + 1) with (Z.succ k) by lia;
+            rewrite Z.pow_succ_r by lia; ring).
+      rewrite Hx.
+      assert (Hfirst_decomp :
+        first = Z.quot first 10 * 10 + Z.rem first 10).
+      {
+        rewrite Z.quot_div_nonneg by lia.
+        rewrite Z.rem_mod_nonneg by lia.
+        pose proof (Z.div_mod first 10 ltac:(lia)).
+        lia.
+      }
+      rewrite Hfirst_decomp at 1.
+      ring.
+Qed.
+
+Lemma special_filter_prefix_init_146 : forall nums,
+  special_filter_prefix_146 nums 0 0.
+Proof.
+  intro nums.
+  unfold special_filter_prefix_146.
+  exists (@nil Z).
+  split; [pose proof (Zlength_nonneg nums); lia|].
+  split.
+  - replace (sublist 0 0 nums) with (@nil Z)
+      by (symmetry; apply sublist_nil; lia).
+    constructor.
+  - reflexivity.
+Qed.
+
+Lemma fold_left_Zadd_app_single_146 : forall scores score,
+  fold_left Z.add (scores ++ [score]) 0 =
+  fold_left Z.add scores 0 + score.
+Proof.
+  intros scores score.
+  rewrite fold_left_app.
+  simpl.
+  lia.
+Qed.
+
+Lemma special_filter_prefix_step_146 : forall nums i count score,
+  0 <= i < Zlength nums ->
+  special_filter_prefix_146 nums i count ->
+  special_number_score (Znth i nums 0) score ->
+  score = 0 \/ score = 1 ->
+  special_filter_prefix_146 nums (i + 1) (count + score).
+Proof.
+  intros nums i count score Hi Hprefix Hscore Hscore01.
+  unfold special_filter_prefix_146 in *.
+  destruct Hprefix as [scores [Hbounds [Hfor Hcount]]].
+  exists (scores ++ [score]).
+  split; [lia|].
+  split.
+  - rewrite (sublist_split 0 (i + 1) i nums)
+      by (try rewrite <- Zlength_correct; lia).
+    rewrite (sublist_single 0 i nums) by lia.
+    apply Forall2_app; [assumption|].
+    constructor; [assumption|constructor].
+  - rewrite fold_left_Zadd_app_single_146.
+    lia.
+Qed.
+
+Lemma special_filter_prefix_step_zero_146 : forall nums i count,
+  0 <= i < Zlength nums ->
+  special_filter_prefix_146 nums i count ->
+  special_number_score (Znth i nums 0) 0 ->
+  special_filter_prefix_146 nums (i + 1) count.
+Proof.
+  intros nums i count Hi Hprefix Hscore.
+  replace count with (count + 0) by lia.
+  eapply special_filter_prefix_step_146; eauto.
+Qed.
+
+Lemma special_filter_prefix_step_one_146 : forall nums i count,
+  0 <= i < Zlength nums ->
+  special_filter_prefix_146 nums i count ->
+  special_number_score (Znth i nums 0) 1 ->
+  special_filter_prefix_146 nums (i + 1) (count + 1).
+Proof.
+  intros nums i count Hi Hprefix Hscore.
+  eapply special_filter_prefix_step_146; eauto.
+Qed.
+
+Lemma special_filter_prefix_final_146 : forall nums count,
+  special_filter_prefix_146 nums (Zlength nums) count ->
+  problem_146_spec_z nums count.
+Proof.
+  intros nums count Hprefix.
+  unfold problem_146_spec_z, problem_146_spec.
+  unfold special_filter_prefix_146 in Hprefix.
+  destruct Hprefix as [scores [Hbounds [Hfor Hcount]]].
+  exists scores.
+  split; [|assumption].
+  replace (sublist 0 (Zlength nums) nums) with nums in Hfor
+    by (symmetry; apply sublist_self; lia).
+  exact Hfor.
+Qed.
+
+Lemma rem10_bounds_146 : forall x,
+  10 < x ->
+  0 <= Z.rem x 10 < 10.
+Proof.
+  intros x Hx.
+  rewrite Z.rem_mod_nonneg by lia.
+  apply Z.mod_pos_bound; lia.
+Qed.
+
+Lemma odd_true_of_rem2_eq1_146 : forall x,
+  0 <= x < 10 ->
+  Z.rem x 2 = 1 ->
+  Z.odd x = true.
+Proof.
+  intros x Hx Hrem.
+  assert (x = 0 \/ x = 1 \/ x = 2 \/ x = 3 \/ x = 4 \/
+          x = 5 \/ x = 6 \/ x = 7 \/ x = 8 \/ x = 9) by lia.
+  repeat (destruct H as [H | H]; [subst; cbn in *; try lia; reflexivity |]);
+    subst; cbn in *; try lia; reflexivity.
+Qed.
+
+Lemma odd_false_of_rem2_neq1_146 : forall x,
+  0 <= x < 10 ->
+  Z.rem x 2 <> 1 ->
+  Z.odd x = false.
+Proof.
+  intros x Hx Hrem.
+  assert (x = 0 \/ x = 1 \/ x = 2 \/ x = 3 \/ x = 4 \/
+          x = 5 \/ x = 6 \/ x = 7 \/ x = 8 \/ x = 9) by lia.
+  repeat (destruct H as [H | H]; [subst; cbn in *; try lia; reflexivity |]);
+    subst; cbn in *; try lia; reflexivity.
+Qed.
+
+Lemma special_score_one_from_scan_146 : forall nums i current first last_digit,
+  special_filter_safe_146 nums ->
+  0 <= i < Zlength nums ->
+  current = Znth i nums 0 ->
+  10 < current ->
+  first_digit_state_146 current first ->
+  first < 10 ->
+  last_digit = Z.rem current 10 ->
+  Z.rem first 2 = 1 ->
+  Z.rem last_digit 2 = 1 ->
+  special_number_score current 1.
+Proof.
+  intros nums i current first last_digit Hsafe Hi Hcur Hgt Hstate Hfirst Hlast Hodd_first Hodd_last.
+  subst current.
+  eapply special_filter_safe_Znth_scan_score_146; eauto.
+  left.
+  repeat split; try lia.
+  - apply odd_true_of_rem2_eq1_146; try lia.
+    destruct Hstate as [Hbounds _]. lia.
+  - apply odd_true_of_rem2_eq1_146; [|assumption].
+    subst last_digit.
+    apply rem10_bounds_146; lia.
+Qed.
+
+Lemma special_score_zero_from_scan_last_146 : forall nums i current first last_digit,
+  special_filter_safe_146 nums ->
+  0 <= i < Zlength nums ->
+  current = Znth i nums 0 ->
+  10 < current ->
+  first_digit_state_146 current first ->
+  first < 10 ->
+  last_digit = Z.rem current 10 ->
+  Z.rem last_digit 2 <> 1 ->
+  special_number_score current 0.
+Proof.
+  intros nums i current first last_digit Hsafe Hi Hcur Hgt Hstate Hfirst Hlast Hodd_last.
+  subst current.
+  eapply special_filter_safe_Znth_scan_score_146; eauto.
+  right.
+  split; [|reflexivity].
+  right; right.
+  apply odd_false_of_rem2_neq1_146; [|assumption].
+  subst last_digit.
+  apply rem10_bounds_146; lia.
+Qed.
+
+Lemma special_score_zero_from_scan_first_146 : forall nums i current first last_digit,
+  special_filter_safe_146 nums ->
+  0 <= i < Zlength nums ->
+  current = Znth i nums 0 ->
+  10 < current ->
+  first_digit_state_146 current first ->
+  first < 10 ->
+  last_digit = Z.rem current 10 ->
+  Z.rem first 2 <> 1 ->
+  special_number_score current 0.
+Proof.
+  intros nums i current first last_digit Hsafe Hi Hcur Hgt Hstate Hfirst Hlast Hodd_first.
+  subst current.
+  eapply special_filter_safe_Znth_scan_score_146; eauto.
+  right.
+  split; [|reflexivity].
+  right; left.
+  apply odd_false_of_rem2_neq1_146; [|assumption].
+  destruct Hstate as [Hbounds _]. lia.
+Qed.
